cosmetic changes and comments

types/coq/SosADL/TypeSystem.v
@@ -9,14 +9,44 @@ Require Import BinInt.
 (** printing Delta $\Delta$ #&Delta;# *)
 (** printing Phi $\Phi$ #&Phi;# *)
 (** printing Gamma $\Gamma$ #&Gamma;# *)
+(** printing Gamma1 $\Gamma_1$ #&Gamma;1# *)
+(** printing Gamma2 $\Gamma_2$ #&Gamma;2# *)
+(** printing Gamma3 $\Gamma_3$ #&Gamma;3# *)
+(** printing Gamma4 $\Gamma_4$ #&Gamma;4# *)
+(** printing Gamma5 $\Gamma_5$ #&Gamma;5# *)
+(** printing Gammap $\Gamma_p$ #&Gamma;p# *)
+(** printing Gammav $\Gamma_v$ #&Gamma;v# *)
 (** printing tau $\tau$ #&tau;# *)
+(** printing tau__e $\tau_e$ #&tau;<sub>e</sub># *)
+(** printing tau__f $\tau_f$ #&tau;<sub>f</sub># *)
+(** printing tau__x $\tau_x$ #&tau;<sub>x</sub># *)
 (** printing Pi $\Pi$ #&Pi;# *)
 (** printing empty $\emptyset$ #&empty;# *)
+(** printing </ $\subseteq$ #&sube;# *)
+(** printing False $\bot$ #&perp;# *)
+(** printing conn__tau $conn_{\tau}$ #conn<sub>&tau;</sub># *)
+(** printing l__tau $l_{\tau}$ #l<sub>&tau;</sub># *)
+(** printing r__tau $r_{\tau}$ #r<sub>&tau;</sub># *)
+(** printing l__min $l_{min}$ #l<sub>min</sub># *)
+(** printing l__max $l_{max}$ #l<sub>max</sub># *)
+(** printing r__min $r_{min}$ #r<sub>min</sub># *)
+(** printing r__max $r_{max}$ #r<sub>max</sub># *)
+(** printing r_min $r_{min}$ #r<sub>min</sub># *)
+(** printing r_max $r_{max}$ #r<sub>max</sub># *)
+(** printing x__min $x_{min}$ #x<sub>min</sub># *)
+(** printing x__max $x_{max}$ #x<sub>max</sub># *)
+(** printing x__min_ $x_{min'}$ #x<sub>min'</sub># *)
+(** printing x__max_ $x_{max'}$ #x<sub>max'</sub># *)
+(** printing x_min $x_{min}$ #x<sub>min</sub># *)
+(** printing x_max $x_{max}$ #x<sub>max</sub># *)
+(** printing x_min_ $x_{min'}$ #x<sub>min'</sub># *)
+(** printing x_max_ $x_{max'}$ #x<sub>max'</sub># *)
 
 (**
 %
 \def\todo#1{{\color{red}TODO: #1}}
 \def\note#1{{\color{blue}NOTE: #1}}
+\def\deprecated#1{{\color{purple}DEPRECATED: #1}}
 %
  *)
 
@@ -49,10 +79,13 @@ objects that can be stored in the typing environment. The main kinds of objects 
 - [EVariable]: value-storing variable
 - [EConnection] a single connection, within a gate or a duty
 
+%\note{%The type system implements structural subtyping. This is the reason why each data type declaration is stored in the environment with a substituting type.%}%
+
  *)
 
 Inductive env_content: Set :=
-| EType: SosADL.SosADL.t_DataTypeDecl -> SosADL.SosADL.t_DataType -> list SosADL.SosADL.t_FunctionDecl -> env_content
+| EType: SosADL.SosADL.t_DataTypeDecl -> SosADL.SosADL.t_DataType
+         -> list SosADL.SosADL.t_FunctionDecl -> env_content
 | ESystem: SosADL.SosADL.t_SystemDecl -> env_content
 | EMediator: SosADL.SosADL.t_MediatorDecl -> env_content
 | EArchitecture: SosADL.SosADL.t_ArchitectureDecl -> env_content
@@ -68,6 +101,16 @@ Definition env := environment env_content.
 
 (**
  ** Communication helpers
+ *)
+
+(** The [connection_defined] predicate states that a connection with
+given properties (name, mode, type and environment) exists in a given
+list.
+
+%\note{%The predicate is expressed as the existence of a rank [i] at
+ which the connection is assumed to exist in the given list. This
+ approach simplifies the generation of the proof, which is here a pair
+ of an integer and an [eq_refl] value.%}%
 *)
 
 Definition connection_defined
@@ -77,9 +120,13 @@ Definition connection_defined
            (mode: SosADL.SosADL.ModeType)
            (tau: SosADL.SosADL.t_DataType)
   := exists (i: Z), match List.nth_error l (Z.to_nat i) with
-               | Some c => c = SosADL.SosADL.Connection (Some is_env) (Some conn) (Some mode) (Some tau)
+               | Some c => c = SosADL.SosADL.Connection
+                                (Some is_env) (Some conn) (Some mode) (Some tau)
                | None => False
                end.
+
+(** [mode_send] and [mode_receive] state the valid connection modes
+for sending and receiving data, respectively.  *)
 
 Inductive mode_send: SosADL.SosADL.ModeType -> Prop :=
 | mode_send_out: mode_send SosADL.SosADL.ModeTypeOut
@@ -93,8 +140,11 @@ Inductive mode_receive: SosADL.SosADL.ModeType -> Prop :=
  ** Method helpers
  *)
 
-(** The following notations is a shortcut to look for a method in a
-data type declaration.  *)
+(** The [method_defined] predicate states that a method with given
+name, self type, return type and formal parameters exist in a given
+list of function declarations. [method_defined'] and
+[method_defined''] are semantically-equivalent alternative definitions
+for this predicate. Their equivalence can be proved. *)
 
 Definition method_defined'
            (m: string)
@@ -156,28 +206,51 @@ Notation "'method' m 'defined' 'in' d 'with' tau 'parameters' f 'returns' r" :=
  ** Field helpers
  *)
 
-(** [field_has_type] is a predicate to look for a field in a list of
-field declarations. *)
+(** [field_has_type] is a predicate that looks for a field with given
+name and type in a list of field declarations. *)
 
-Inductive field_has_type: list SosADL.SosADL.t_FieldDecl -> string -> SosADL.SosADL.t_DataType -> Prop :=
-| First_Field: forall n t r, field_has_type (SosADL.SosADL.FieldDecl (Some n) (Some t) :: r) n t
-| Next_Field: forall n t h r, field_has_type r n t -> field_has_type (h :: r) n t.
+Inductive field_has_type:
+  list SosADL.SosADL.t_FieldDecl -> string -> SosADL.SosADL.t_DataType -> Prop :=
+| First_Field:
+    forall n t r,
+      field_has_type (SosADL.SosADL.FieldDecl (Some n) (Some t) :: r) n t
+                     
+| Next_Field:
+    forall n t h r,
+      field_has_type r n t -> field_has_type (h :: r) n t.
 
-Fixpoint field_type (l: list SosADL.SosADL.t_FieldDecl) (n: string) {struct l}: option SosADL.SosADL.t_DataType :=
+(** [field_type] is a function that returns the type of a field given
+by its name. *)
+
+Fixpoint field_type (l: list SosADL.SosADL.t_FieldDecl) (n: string) {struct l}:
+  option SosADL.SosADL.t_DataType :=
   match l with
   | nil => None
-  | (SosADL.SosADL.FieldDecl (Some f) r) :: tl => if string_dec n f then r else field_type tl n
+  | (SosADL.SosADL.FieldDecl (Some f) r) :: tl =>
+    if string_dec n f then r else field_type tl n
   | _ :: tl => field_type tl n
   end.
-
-(*Hypothesis names_of_expression: SosADL.SosADL.t_Expression -> list string.*)
 
 
 (** * Subtyping relation *)
 
 Reserved Notation "t1 </ t2" (at level 70).
 
-Inductive subtype: SosADL.SosADL.t_DataType -> SosADL.SosADL.t_DataType -> Prop :=
+(** The [subtype] relation states whenever a type is included in
+another type. Inclusion is here understood as the inclusion of the
+sets of values corresponding to the types, which is especially
+meaningful for range types. Tuple and sequence types are covariant.
+Moreover, a tuple type is included in another tuple type if and only
+if it declares the same fields possibly with additional ones.
+
+%\note{%The [subtype] relation, like the reminder of the type system,
+ implements structural subtyping. This is the reason why no subtyping
+ rule applies to named types, except [subtype_refl], the reflectivity
+ rule.%}% *)
+
+Inductive subtype:
+  SosADL.SosADL.t_DataType -> SosADL.SosADL.t_DataType -> Prop :=
+  
 | subtype_refl:
     forall
       (t: SosADL.SosADL.t_DataType)
@@ -193,7 +266,8 @@ Inductive subtype: SosADL.SosADL.t_DataType -> SosADL.SosADL.t_DataType -> Prop 
       (p1: rmi <= lmi)
       (p2: lma <= rma)
     ,
-      (SosADL.SosADL.RangeType (Some lmi) (Some lma)) </ (SosADL.SosADL.RangeType (Some rmi) (Some rma))
+      (SosADL.SosADL.RangeType (Some lmi) (Some lma))
+        </ (SosADL.SosADL.RangeType (Some rmi) (Some rma))
 
 | subtype_tuple:
     forall (l: list SosADL.SosADL.t_FieldDecl)
@@ -213,17 +287,19 @@ Inductive subtype: SosADL.SosADL.t_DataType -> SosADL.SosADL.t_DataType -> Prop 
       (r: SosADL.SosADL.t_DataType)
       (p1: l </ r)
     ,
-      (SosADL.SosADL.SequenceType (Some l)) </ (SosADL.SosADL.SequenceType (Some r))
+      (SosADL.SosADL.SequenceType (Some l))
+        </ (SosADL.SosADL.SequenceType (Some r))
 
 where "t1 </ t2" := (subtype t1 t2)
 .
 
-(**
- * Generic constructions
+(** * Generic constructions
 
-The following provide generic constructions for the type system.
+The following definitions provide generic constructions for the type
+system, especially to deal with definitions and with optionality.
 
- *)
+[augment_env] is a function that optionally binds a new name in an
+environment.  *)
 
 Definition augment_env (Gamma: env) (n: option string) (c: option env_content) :=
   match n with
@@ -235,7 +311,10 @@ Definition augment_env (Gamma: env) (n: option string) (c: option env_content) :
     end
   end.
 
-(** [incrementally] is a generic set of rules for incremental, ordered definitions. *)
+(** [incrementally] is a generic set of rules for incremental ordered
+definitions, i.e., each definition can be used in subsequent
+definitions. [incrementally] can be proved to fold the list in the
+same way as [fold_left]. *)
 
 Inductive incrementally
           {T: Set} {P: env -> T -> env -> Prop}:
@@ -260,6 +339,11 @@ Inductive incrementally
       incrementally Gamma (x::l) Gamma1
 .
 
+(** A [simple_increment] is to be used in conjunction with
+[incrementally] in order to implement its [P] parameter when it made
+of a proof of an (arbitrary) property along with a call to
+[augment_env]. *)
+
 Inductive simple_increment
           (T: Set) (P: env -> T -> Prop) (name: T -> option string)
           (content: T -> option env_content):
@@ -276,40 +360,25 @@ Inductive simple_increment
       simple_increment T P name content Gamma x Gamma1
 .
 
-Lemma incrementally_fold_left:
-  forall {T: Set} (P: env -> T -> env -> Prop) (name: T -> option string)
-         (content: T -> option env_content)
-         (p: forall g x g', P g x g' -> g' = augment_env g (name x) (content x))
-         (l: list T)
-         (Gamma: env) (Gamma': env)
-         (s: @incrementally T P Gamma l Gamma'),
-    Gamma' = fold_left (fun r x => augment_env r (name x) (content x)) l Gamma.
-Proof.
-  intros.
-  induction s.
-  - auto.
-  - apply p in p1. subst. auto.
-Qed.
+(** [augment_env_with_all] binds a list of names in an
+environment. This function is intended to be used in conjunction with
+[mutually]: it assumes that the order in which the names are bound is
+irrelevant.
 
-Lemma simple_incrementally_fold_left:
-  forall {T: Set} (P: env -> T -> Prop) (name: T -> option string)
-         (content: T -> option env_content)
-         (l: list T)
-         (Gamma: env) (Gamma': env)
-         (s: @incrementally T (simple_increment T P name content) Gamma l Gamma'),
-    Gamma' = fold_left (fun r x => augment_env r (name x) (content x)) l Gamma.
-Proof.
-  intros T P name content l Gamma Gamma'. apply incrementally_fold_left. intros g x g' H.
-  destruct H. auto.
-Qed.
+%\note{%The implementation uses [fold_right] because it is
+ tail-recursive.%}% *)
 
-Definition augment_env_with_all (Gamma: env) {T: Set} (name: T -> option string) (content: T -> option env_content) (l: list T) :=
+Definition augment_env_with_all
+           (Gamma: env) {T: Set} (name: T -> option string)
+           (content: T -> option env_content) (l: list T) :=
   List.fold_right (fun x g => augment_env g (name x) (content x)) Gamma l.
 
-(** [mutually] is a generic rule for unordered, simultaneous, mutual definitions. *)
+(** [mutually] is a generic rule for unordered, simultaneous, mutual
+definitions that can refer to each other. *)
 
 Inductive mutually
-          {T: Set} {P: env -> T -> env -> Prop} {name: T -> option string} {content: T -> option env_content}:
+          {T: Set} {P: env -> T -> env -> Prop} {name: T -> option string}
+          {content: T -> option env_content}:
   env -> list T -> env -> Prop :=
 
 | mutually_all:
@@ -324,10 +393,15 @@ Inductive mutually
       mutually Gamma l Gamma1
 .
 
-(** [mutually_translate] is a generic rule for unordered, simultaneous, mutual definitions. *)
+(** [mutually_translate] is a generic rule for unordered,
+simultaneous, mutual definitions that can refer to each other. The
+difference between [mutually] and [mutually_translate] is that the
+latter offers the opportunity to translate the items added to the
+environment. *)
 
 Inductive mutually_translate
-          {T: Set} {P: env -> T -> T -> env -> Prop} {name: T -> option string} {content: T -> option env_content}:
+          {T: Set} {P: env -> T -> T -> env -> Prop} {name: T -> option string}
+          {content: T -> option env_content}:
   env -> list T -> list T -> env -> Prop :=
 
 | mutually_translate_all:
@@ -343,7 +417,8 @@ Inductive mutually_translate
       mutually_translate Gamma l l1 Gamma1
 .
 
-(** [optionally] is a generic rule for an optional statement. *)
+(** [optionally] is a generic rule that proves an optional
+statement. *)
 
 Inductive optionally {T: Set} {P: env -> T -> Prop}:
   env -> option T -> Prop :=
@@ -362,33 +437,30 @@ Inductive optionally {T: Set} {P: env -> T -> Prop}:
       optionally Gamma (Some x)
 .
 
-(**
- * Notations
+(** * Notations
 
-The following notations defines all the judgment forms in the type
-system. Usually, the typing environment is denoted [Gamma].
+** Judgements
 
-The judgement for statements ([body]) has a second environment denoted
-[Pi], holding the types of the formal parameters of the enclosing
-behavior. This second environment [Pi] is mandatory to type the
-recursive call statement.
+The following notations define all the judgment forms in the type
+system. Usually, the environment is denoted [Gamma].  *)
 
- *)
-
-Reserved Notation "'expression' e 'is' 'constant' 'integer'" (at level 200, no associativity).
+Reserved Notation "'expression' e 'is' 'constant' 'integer'"
+         (at level 200, no associativity).
 Reserved Notation "'SoSADL' a 'well' 'typed'" (at level 200, no associativity).
 Reserved Notation "'unit' u 'well' 'typed' 'in' Gamma" (at level 200, no associativity).
 Reserved Notation "'entity' u 'well' 'typed' 'in' Gamma" (at level 200, Gamma at level 1, no associativity).
 Reserved Notation "'typedecl' t 'well' 'typed' 'in' Gamma 'yields' 'to' Gamma1" (at level 200, Gamma at level 1, no associativity).
 Reserved Notation "'function' f 'well' 'typed' 'in' Gamma 'yields' 'to' Gamma1" (at level 200, Gamma at level 1, no associativity).
 Reserved Notation "'type' t 'looks' 'fine'" (at level 200, no associativity).
-Reserved Notation "'type' t 'is' u 'in' Gamma" (at level 200, Gamma at level 1, no associativity).
+Reserved Notation "'type' t 'is' u 'in' Gamma"
+         (at level 200, Gamma at level 1, no associativity).
 Reserved Notation "'system' s 'well' 'typed' 'in' Gamma" (at level 200, Gamma at level 1, no associativity).
 Reserved Notation "'mediator' m 'well' 'typed' 'in' Gamma" (at level 200, Gamma at level 1, no associativity).
 Reserved Notation "'mediatorblock' m 'well' 'typed' 'in' Gamma" (at level 200, Gamma at level 1, no associativity).
 Reserved Notation "'architecture' a 'well' 'typed' 'in' Gamma" (at level 200, Gamma at level 1, no associativity).
 Reserved Notation "'architectureblock' a 'well' 'typed' 'in' Gamma" (at level 200, Gamma at level 1, no associativity).
-Reserved Notation "'expression' e 'has' 'type' t 'in' Gamma" (at level 200, no associativity, Gamma at level 1).
+Reserved Notation "'expression' e 'has' 'type' t 'in' Gamma"
+         (at level 200, no associativity, Gamma at level 1).
 Reserved Notation "'expression' 'node' e 'has' 'type' t 'in' Gamma" (at level 200, no associativity, Gamma at level 1).
 Reserved Notation "'archbehavior' b 'well' 'typed' 'in' Gamma" (at level 200, Gamma at level 1, no associativity).
 Reserved Notation "'behavior' b 'well' 'typed' 'in' Gamma" (at level 200, Gamma at level 1, no associativity).
@@ -397,27 +469,77 @@ Reserved Notation "'protocol' p 'well' 'typed' 'in' Gamma" (at level 200, Gamma 
 Reserved Notation "'final' 'body' b 'well' 'typed' 'in' Gamma" (at level 200, Gamma at level 1, no associativity).
 Reserved Notation "'statement' b 'well' 'typed' 'in' Gamma 'yields' 'to' Gamma1" (at level 200, Gamma at level 1, no associativity).
 Reserved Notation "'nonfinal' 'body' b 'well' 'typed' 'in' Gamma" (at level 200, Gamma at level 1, no associativity).
-Reserved Notation "'valuing' v 'well' 'typed' 'in' Gamma 'yields' 'to' Gamma1" (at level 200, Gamma at level 1, no associativity).
+Reserved Notation "'valuing' v 'well' 'typed' 'in' Gamma 'yields' 'to' Gamma1" (at level 200, Gamma at level 1, v at level 1, no associativity).
+
+(**
+ ** SoSADL notations
+ *)
+
+(** The [sosadl_scope] notation scope and [%sosadl] key are used to
+provide convenient notations for SoSADL expressions.  *)
+
+Import ListNotations.
+Local Open Scope list_scope.
+Local Open Scope string_scope.
+Delimit Scope sosadl_scope with sosadl.
+
+Notation "- x" := (SosADL.SosADL.UnaryExpression (Some "-") (Some x)) : sosadl_scope.
+Notation "+ x" := (SosADL.SosADL.UnaryExpression (Some "+") (Some x)) (at level 35, x at level 35) : sosadl_scope.
+
+Notation "l * r" := (SosADL.SosADL.BinaryExpression (Some l) (Some "*") (Some r)) : sosadl_scope.
+Notation "l / r" := (SosADL.SosADL.BinaryExpression (Some l) (Some "/") (Some r)) : sosadl_scope.
+Notation "l 'mod' r" :=
+  (SosADL.SosADL.BinaryExpression (Some l) (Some "mod") (Some r)) : sosadl_scope.
+
+Notation "l + r" := (SosADL.SosADL.BinaryExpression (Some l) (Some "+") (Some r)) : sosadl_scope.
+Notation "l - r" := (SosADL.SosADL.BinaryExpression (Some l) (Some "-") (Some r)) : sosadl_scope.
+
+Notation "l < r" := (SosADL.SosADL.BinaryExpression (Some l) (Some "<") (Some r)) : sosadl_scope.
+Notation "l <= r" := (SosADL.SosADL.BinaryExpression (Some l) (Some "<=") (Some r)) : sosadl_scope.
+Notation "l > r" := (SosADL.SosADL.BinaryExpression (Some l) (Some ">") (Some r)) : sosadl_scope.
+Notation "l >= r" := (SosADL.SosADL.BinaryExpression (Some l) (Some ">=") (Some r)) : sosadl_scope.
+Notation "l = r" := (SosADL.SosADL.BinaryExpression (Some l) (Some "=") (Some r)) : sosadl_scope.
+Notation "l <> r" := (SosADL.SosADL.BinaryExpression (Some l) (Some "<>") (Some r)) : sosadl_scope.
+
+Notation "l '->' r" := (SosADL.SosADL.BinaryExpression (Some l) (Some "implies") (Some r)) : sosadl_scope.
+Notation "l '&&' r" := (SosADL.SosADL.BinaryExpression (Some l) (Some "and") (Some r)) : sosadl_scope.
+Notation "l '||' r" := (SosADL.SosADL.BinaryExpression (Some l) (Some "or") (Some r)) : sosadl_scope.
+Notation "l '^^' r" := (SosADL.SosADL.BinaryExpression (Some l) (Some "xor") (Some r)) (at level 50, left associativity) : sosadl_scope.
+Notation "! x" := (SosADL.SosADL.UnaryExpression (Some "not") (Some x)) (at level 35, x at level 35) : sosadl_scope.
+
+Notation "[ l , r ]" := (SosADL.SosADL.RangeType (Some l) (Some r)) (at level 0, l at level 200, r at level 200) : sosadl_scope.
+
+Notation "s :: { x -> e }" := (SosADL.SosADL.Map (Some s) (Some x) (Some e)) (at level 59, x at level 1, e at level 200, left associativity) : sosadl_scope.
+Notation "s :: { x | e }" := (SosADL.SosADL.Select (Some s) (Some x) (Some e)) (at level 59, x at level 1, e at level 200, left associativity) : sosadl_scope.
+
+Notation "s ::: f" := (SosADL.SosADL.Field (Some s) (Some f)) (at level 59, f at level 1, left associativity) : sosadl_scope.
+
+Notation "'valuing' x = e" := (SosADL.SosADL.Valuing (Some x) None (Some e)) (at level 200, x at level 1) : sosadl_scope.
+Notation "'valuing' x 'is' t = e" := (SosADL.SosADL.Valuing (Some x) (Some t) (Some e)) (at level 200, x at level 1, t at level 1) : sosadl_scope.
 
 (**
  * The type system
  *)
-
-Local Open Scope list_scope.
-Local Open Scope string_scope.
 
 (** In the following rules, each inductive type gathers the rules for
 a single form of judgment. Rules are built of the following:
 
 - a rule name, here used as the name of the constructor in the inductive type;
 - universal quantification of the free names of the rules;
-- premises of the rule appear above the [->] operator, connected by the conjunction [/\] operator; and
-- conclusion of the rule appear below the [->] operator.
+- premises of the rule appear as additional parameters whose name usually starts with [p]; and
+- conclusion of the rule appear below the [,].
  *)
 
 (**
  ** Constant expressions
  *)
+
+(** The [constexpr_expression] predicate states that an expression is
+manifestly constant. It is based on a syntactical criterion.
+
+%\deprecated{%The criterion is overly strict as it does not allow (for
+ instance) the use of literal tuples nor sequences. This predicate is
+ not used in the type system.%}% *)
 
 Inductive constexpr_expression: SosADL.SosADL.t_Expression -> Prop :=
 | constexpr_IntegerValue:
@@ -431,14 +553,14 @@ Inductive constexpr_expression: SosADL.SosADL.t_Expression -> Prop :=
       (e: SosADL.SosADL.t_Expression)
       (p: expression e is constant integer)
     ,
-      expression (SosADL.SosADL.UnaryExpression (Some "-") (Some e)) is constant integer
+      expression (- e)%sosadl is constant integer
 
 | constexpr_Same:
     forall
       (e: SosADL.SosADL.t_Expression)
       (p: expression e is constant integer)
     ,
-      expression (SosADL.SosADL.UnaryExpression (Some "+") (Some e)) is constant integer
+      expression (+ e)%sosadl is constant integer
 
 | constexpr_Add:
     forall
@@ -447,7 +569,7 @@ Inductive constexpr_expression: SosADL.SosADL.t_Expression -> Prop :=
       (p1: expression l is constant integer)
       (p2: expression r is constant integer)
     ,
-      expression (SosADL.SosADL.BinaryExpression (Some l) (Some "+") (Some r)) is constant integer
+      expression (l + r)%sosadl is constant integer
 
 | constexpr_Sub:
     forall
@@ -456,7 +578,7 @@ Inductive constexpr_expression: SosADL.SosADL.t_Expression -> Prop :=
       (p1: expression l is constant integer)
       (p2: expression r is constant integer)
     ,
-      expression (SosADL.SosADL.BinaryExpression (Some l) (Some "-") (Some r)) is constant integer
+      expression (l - r)%sosadl is constant integer
 
 | constexpr_Mul:
     forall
@@ -465,7 +587,7 @@ Inductive constexpr_expression: SosADL.SosADL.t_Expression -> Prop :=
       (p1: expression l is constant integer)
       (p2: expression r is constant integer)
     ,
-      expression (SosADL.SosADL.BinaryExpression (Some l) (Some "*") (Some r)) is constant integer
+      expression (l * r)%sosadl is constant integer
 
 | constexpr_Div:
     forall
@@ -474,7 +596,7 @@ Inductive constexpr_expression: SosADL.SosADL.t_Expression -> Prop :=
       (p1: expression l is constant integer)
       (p2: expression r is constant integer)
     ,
-      expression (SosADL.SosADL.BinaryExpression (Some l) (Some "/") (Some r)) is constant integer
+      expression (l / r)%sosadl is constant integer
 
 | constexpr_Mod:
     forall
@@ -483,12 +605,22 @@ Inductive constexpr_expression: SosADL.SosADL.t_Expression -> Prop :=
       (p1: expression l is constant integer)
       (p2: expression r is constant integer)
     ,
-      expression (SosADL.SosADL.BinaryExpression (Some l) (Some "mod") (Some r)) is constant integer
+      expression (l mod r)%sosadl is constant integer
                  
 where "'expression' e 'is' 'constant' 'integer'" := (constexpr_expression e)
 .
 
-(** ** Data types *)
+(** ** Data types
+
+The [check_datatype] predicate asserts that a data type is valid. A
+data type is said valid if and only if, when it is a range type, the
+lower bound is smaller than or equal to the upper bound according to
+some interpretation. Tuple type and sequence type are valid if the
+item types are valid as well. Named type and boolean type are always
+valid.
+
+%\note{%In the case of range type, their interpretation ensures that
+the bounds are integer.%}% *)
 
 Inductive check_datatype: SosADL.SosADL.t_DataType -> Prop :=
 | check_NamedType:
@@ -500,9 +632,11 @@ Inductive check_datatype: SosADL.SosADL.t_DataType -> Prop :=
 | check_TupleType:
     forall
       (fields: list SosADL.SosADL.t_FieldDecl)
-      (p1: values (SosADL.SosADL.FieldDecl_name f) for f of fields are distinct according to option_string_dec)
-      (p2: for each f of fields, exists t, SosADL.SosADL.FieldDecl_type f = Some t
-                                      /\ type t looks fine)
+      (p1: values (SosADL.SosADL.FieldDecl_name f) for f of fields
+                  are distinct according to option_string_dec)
+      (p2: for each f of fields,
+           exists t, (SosADL.SosADL.FieldDecl_type f = Some t
+                 /\ type t looks fine))
     ,
       type (SosADL.SosADL.TupleType fields) looks fine
 
@@ -519,8 +653,7 @@ Inductive check_datatype: SosADL.SosADL.t_DataType -> Prop :=
       (max: SosADL.SosADL.t_Expression)
       (p1: min <= max)
     ,
-      type (SosADL.SosADL.RangeType (Some min)
-                                    (Some max)) looks fine
+      type [min, max]%sosadl looks fine
 
 | check_BooleanType:
       type SosADL.SosADL.BooleanType looks fine
@@ -528,7 +661,18 @@ Inductive check_datatype: SosADL.SosADL.t_DataType -> Prop :=
 where "'type' t 'looks' 'fine'" := (check_datatype t)
 .
 
-Inductive type_datatype: env -> SosADL.SosADL.t_DataType -> SosADL.SosADL.t_DataType -> Prop :=
+(** [type_datatype] is a predicate that asserts that a data type is
+correct in a given environment and that, according to this
+environment, it should be substituted by a given data type.
+
+Substitution occurs recursively in the data type. Whenever a named
+type is found, it is substituted as found in the environment.
+
+%\note{%Type substitution is part of the mechanics that implements
+ structural typing.%}% *)
+
+Inductive type_datatype:
+  env -> SosADL.SosADL.t_DataType -> SosADL.SosADL.t_DataType -> Prop :=
 | type_NamedType:
     forall
       (Gamma: env)
@@ -544,14 +688,16 @@ Inductive type_datatype: env -> SosADL.SosADL.t_DataType -> SosADL.SosADL.t_Data
       (Gamma: env)
       (fields: list SosADL.SosADL.t_FieldDecl)
       (fields': list SosADL.SosADL.t_FieldDecl)
-      (p1: values (SosADL.SosADL.FieldDecl_name f) for f of fields are distinct according to option_string_dec)
+      (p1: values (SosADL.SosADL.FieldDecl_name f) for f of fields
+                  are distinct according to option_string_dec)
       (p2: for each f f' of fields fields',
            SosADL.SosADL.FieldDecl_name f = SosADL.SosADL.FieldDecl_name f'
            /\ exists t, SosADL.SosADL.FieldDecl_type f = Some t
                   /\ exists t', SosADL.SosADL.FieldDecl_type f' = Some t'
-                                      /\ type t is t' in Gamma)
+                          /\ type t is t' in Gamma)
     ,
-      type (SosADL.SosADL.TupleType fields) is (SosADL.SosADL.TupleType fields') in Gamma
+      type (SosADL.SosADL.TupleType fields)
+           is (SosADL.SosADL.TupleType fields') in Gamma
 
 | type_SequenceType:
     forall
@@ -560,7 +706,8 @@ Inductive type_datatype: env -> SosADL.SosADL.t_DataType -> SosADL.SosADL.t_Data
       (t': SosADL.SosADL.t_DataType)
       (p: type t is t' in Gamma)
     ,
-      type (SosADL.SosADL.SequenceType (Some t)) is (SosADL.SosADL.SequenceType (Some t')) in Gamma
+      type (SosADL.SosADL.SequenceType (Some t))
+           is (SosADL.SosADL.SequenceType (Some t')) in Gamma
 
 | type_RangeType_trivial:
     forall
@@ -569,10 +716,7 @@ Inductive type_datatype: env -> SosADL.SosADL.t_DataType -> SosADL.SosADL.t_Data
       (max: SosADL.SosADL.t_Expression)
       (p1: min <= max)
     ,
-      type (SosADL.SosADL.RangeType (Some min)
-                                    (Some max))
-           is (SosADL.SosADL.RangeType (Some min)
-                                       (Some max)) in Gamma
+      type [min, max]%sosadl is [min, max]%sosadl in Gamma
 
 | type_BooleanType:
     forall
@@ -583,14 +727,20 @@ Inductive type_datatype: env -> SosADL.SosADL.t_DataType -> SosADL.SosADL.t_Data
 where "'type' t 'is' u 'in' Gamma" := (type_datatype Gamma t u)
 .
 
-(**
- ** Expression
+(** ** Expression
 
-Before running into the type system for expressions, we first introduce some definitions and properties about interval arithmetic.
+Before running into the type system for expressions, we first
+introduce some definitions and properties about interval arithmetic,
+and more specifically for the [mod] operator:
 
+- [range_modulo_min] asserts the suitable lower bound;
+- [range_modulo_max] the suitable upper bound.
  *)
 
-Inductive range_modulo_min: SosADL.SosADL.t_Expression -> SosADL.SosADL.t_Expression -> SosADL.SosADL.t_Expression -> SosADL.SosADL.t_Expression -> SosADL.SosADL.t_Expression -> Prop :=
+Inductive range_modulo_min:
+  SosADL.SosADL.t_Expression -> SosADL.SosADL.t_Expression
+  -> SosADL.SosADL.t_Expression -> SosADL.SosADL.t_Expression
+  -> SosADL.SosADL.t_Expression -> Prop :=
 | range_modulo_min_pos:
     forall
       (lmin: SosADL.SosADL.t_Expression)
@@ -599,7 +749,7 @@ Inductive range_modulo_min: SosADL.SosADL.t_Expression -> SosADL.SosADL.t_Expres
       (rmax: SosADL.SosADL.t_Expression)
       (min: SosADL.SosADL.t_Expression)
       (p1: (SosADL.SosADL.IntegerValue (Some 1%Z)) <= rmin)
-      (p2: min <= (SosADL.SosADL.BinaryExpression (Some (SosADL.SosADL.IntegerValue (Some 1%Z))) (Some "-") (Some rmax)))
+      (p2: min <= ((SosADL.SosADL.IntegerValue (Some 1%Z)) - rmax)%sosadl)
     ,
       range_modulo_min lmin lmax rmin rmax min
 
@@ -622,13 +772,16 @@ Inductive range_modulo_min: SosADL.SosADL.t_Expression -> SosADL.SosADL.t_Expres
       (rmin: SosADL.SosADL.t_Expression)
       (rmax: SosADL.SosADL.t_Expression)
       (min: SosADL.SosADL.t_Expression)
-      (p1: rmax <= (SosADL.SosADL.UnaryExpression (Some "-") (Some (SosADL.SosADL.IntegerValue (Some 1%Z)))))
-      (p2: min <= (SosADL.SosADL.BinaryExpression (Some rmin) (Some "+") (Some (SosADL.SosADL.IntegerValue (Some 1%Z)))))
+      (p1: rmax <= (- (SosADL.SosADL.IntegerValue (Some 1%Z)))%sosadl)
+      (p2: min <= (rmin + (SosADL.SosADL.IntegerValue (Some 1%Z)))%sosadl)
     ,
       range_modulo_min lmin lmax rmin rmax min
 .
 
-Inductive range_modulo_max: SosADL.SosADL.t_Expression -> SosADL.SosADL.t_Expression -> SosADL.SosADL.t_Expression -> SosADL.SosADL.t_Expression -> SosADL.SosADL.t_Expression -> Prop :=
+Inductive range_modulo_max:
+  SosADL.SosADL.t_Expression -> SosADL.SosADL.t_Expression
+  -> SosADL.SosADL.t_Expression -> SosADL.SosADL.t_Expression
+  -> SosADL.SosADL.t_Expression -> Prop :=
 | range_modulo_max_pos:
     forall
       (lmin: SosADL.SosADL.t_Expression)
@@ -637,7 +790,7 @@ Inductive range_modulo_max: SosADL.SosADL.t_Expression -> SosADL.SosADL.t_Expres
       (rmax: SosADL.SosADL.t_Expression)
       (max: SosADL.SosADL.t_Expression)
       (p1: (SosADL.SosADL.IntegerValue (Some 1%Z)) <= rmin)
-      (p2: (SosADL.SosADL.BinaryExpression (Some rmax) (Some "-") (Some (SosADL.SosADL.IntegerValue (Some 1%Z)))) <= max)
+      (p2: (rmax - (SosADL.SosADL.IntegerValue (Some 1%Z)))%sosadl <= max)
     ,
       range_modulo_max lmin lmax rmin rmax max
 
@@ -660,18 +813,31 @@ Inductive range_modulo_max: SosADL.SosADL.t_Expression -> SosADL.SosADL.t_Expres
       (rmin: SosADL.SosADL.t_Expression)
       (rmax: SosADL.SosADL.t_Expression)
       (max: SosADL.SosADL.t_Expression)
-      (p1: rmax <= (SosADL.SosADL.UnaryExpression (Some "-") (Some (SosADL.SosADL.IntegerValue (Some 1%Z)))))
-      (p2: (SosADL.SosADL.BinaryExpression (Some (SosADL.SosADL.UnaryExpression (Some "-") (Some (SosADL.SosADL.IntegerValue (Some 1%Z))))) (Some "-") (Some rmin)) <= max)
+      (p1: rmax <= (- (SosADL.SosADL.IntegerValue (Some 1%Z)))%sosadl)
+      (p2: ((- (SosADL.SosADL.IntegerValue (Some 1%Z))) - rmin)%sosadl <= max)
     ,
       range_modulo_max lmin lmax rmin rmax max
 .
 
-(*
-%\note{%This set of rules is restricted to computable expressions. This means that [any] and unifications are excluded from these rules. It indeed seems reasonnable,
-at least as a first step, that [any] is allowed solely in the protocols and assertions. %}%
-*)
+(** [type_expression] asserts that an expression has a given type in a
+given environment. This judgment is suitable for computable
+expression, i.e., it does not allow [any] nor [unify] operators. It can be used in the following contexts:
 
-Inductive type_expression: env -> SosADL.SosADL.t_Expression -> SosADL.SosADL.t_DataType -> Prop :=
+- expressions used as range type boundaries;
+- expressions in valuings;
+- expressions in function bodies;
+- expressions in do statements;
+- expressions in send statements.
+
+The rules are structured in two sets of mutually recursive judgements:
+
+- [type_expression] is the callable judgement. It checks that the given type is valid as well.
+- [type_expression_node] contains the actual typing rules.
+ *)
+
+Inductive type_expression:
+  env -> SosADL.SosADL.t_Expression -> SosADL.SosADL.t_DataType -> Prop :=
+  
 | type_expression_and_type:
     forall
       (Gamma: env)
@@ -682,7 +848,8 @@ Inductive type_expression: env -> SosADL.SosADL.t_Expression -> SosADL.SosADL.t_
     ,
       expression e has type t in Gamma
 
-with type_expression_node: env -> SosADL.SosADL.t_Expression -> SosADL.SosADL.t_DataType -> Prop :=
+with type_expression_node:
+       env -> SosADL.SosADL.t_Expression -> SosADL.SosADL.t_DataType -> Prop :=
                       
 | type_expression_IntegerValue:
     forall
@@ -690,9 +857,8 @@ with type_expression_node: env -> SosADL.SosADL.t_Expression -> SosADL.SosADL.t_
       (v: BinInt.Z)
     ,
       expression node (SosADL.SosADL.IntegerValue (Some v))
-      has type (SosADL.SosADL.RangeType
-                  (Some (SosADL.SosADL.IntegerValue (Some v)))
-                  (Some (SosADL.SosADL.IntegerValue (Some v)))) in Gamma
+                 has type [(SosADL.SosADL.IntegerValue (Some v)),
+                           (SosADL.SosADL.IntegerValue (Some v))]%sosadl in Gamma
 
 | type_expression_Opposite:
     forall
@@ -702,12 +868,9 @@ with type_expression_node: env -> SosADL.SosADL.t_Expression -> SosADL.SosADL.t_
       (min: SosADL.SosADL.t_Expression)
       (max: SosADL.SosADL.t_Expression)
       (p1: expression e has type tau in Gamma)
-      (p2: tau </ (SosADL.SosADL.RangeType (Some min) (Some max)))
+      (p2: tau </ [min, max]%sosadl)
     ,
-      expression node (SosADL.SosADL.UnaryExpression (Some "-") (Some e))
-                 has type (SosADL.SosADL.RangeType
-                             (Some (SosADL.SosADL.UnaryExpression (Some "-") (Some max)))
-                             (Some (SosADL.SosADL.UnaryExpression (Some "-") (Some min)))) in Gamma
+      expression node (- e)%sosadl has type [- max, - min]%sosadl in Gamma
 
 | type_expression_Same:
     forall
@@ -717,10 +880,9 @@ with type_expression_node: env -> SosADL.SosADL.t_Expression -> SosADL.SosADL.t_
       (min: SosADL.SosADL.t_Expression)
       (max: SosADL.SosADL.t_Expression)
       (p1: expression e has type tau in Gamma)
-      (p2: tau </ (SosADL.SosADL.RangeType (Some min) (Some max)))
+      (p2: tau </ [min, max]%sosadl)
     ,
-      expression node (SosADL.SosADL.UnaryExpression (Some "+") (Some e))
-      has type (SosADL.SosADL.RangeType (Some min) (Some max)) in Gamma
+      expression node (+ e)%sosadl has type [min, max]%sosadl in Gamma
 
 
 | type_expression_Not:
@@ -731,7 +893,7 @@ with type_expression_node: env -> SosADL.SosADL.t_Expression -> SosADL.SosADL.t_
       (p1: expression e has type tau in Gamma)
       (p2: tau </ SosADL.SosADL.BooleanType)
     ,
-      expression node (SosADL.SosADL.UnaryExpression (Some "not") (Some e)) has type SosADL.SosADL.BooleanType in Gamma
+      expression node (! e)%sosadl has type SosADL.SosADL.BooleanType in Gamma
 
 | type_expression_Add:
     forall
@@ -745,13 +907,12 @@ with type_expression_node: env -> SosADL.SosADL.t_Expression -> SosADL.SosADL.t_
       (r__min: SosADL.SosADL.t_Expression)
       (r__max: SosADL.SosADL.t_Expression)
       (p1: expression l has type l__tau in Gamma)
-      (p2: l__tau </ (SosADL.SosADL.RangeType (Some l__min) (Some l__max)))
+      (p2: l__tau </ [l__min, l__max]%sosadl)
       (p3: expression r has type r__tau in Gamma)
-      (p4: r__tau </ (SosADL.SosADL.RangeType (Some r__min) (Some r__max)))
+      (p4: r__tau </ [r__min, r__max]%sosadl)
     ,
-      expression node (SosADL.SosADL.BinaryExpression (Some l) (Some "+") (Some r))
-      has type (SosADL.SosADL.RangeType (Some (SosADL.SosADL.BinaryExpression (Some l__min) (Some "+") (Some r__min)))
-                              (Some (SosADL.SosADL.BinaryExpression (Some l__max) (Some "+") (Some r__max)))) in Gamma
+      expression node (l + r)%sosadl
+                 has type [ l__min + r__min, l__max + r__max ]%sosadl in Gamma
 
 | type_expression_Sub:
     forall
@@ -765,13 +926,12 @@ with type_expression_node: env -> SosADL.SosADL.t_Expression -> SosADL.SosADL.t_
       (r__min: SosADL.SosADL.t_Expression)
       (r__max: SosADL.SosADL.t_Expression)
       (p1: expression l has type l__tau in Gamma)
-      (p2: l__tau </ (SosADL.SosADL.RangeType (Some l__min) (Some l__max)))
+      (p2: l__tau </ [l__min, l__max]%sosadl)
       (p3: expression r has type r__tau in Gamma)
-      (p4: r__tau </ (SosADL.SosADL.RangeType (Some r__min) (Some r__max)))
+      (p4: r__tau </ [r__min, r__max]%sosadl)
     ,
-      expression node (SosADL.SosADL.BinaryExpression (Some l) (Some "-") (Some r))
-      has type (SosADL.SosADL.RangeType (Some (SosADL.SosADL.BinaryExpression (Some l__min) (Some "-") (Some r__max)))
-                              (Some (SosADL.SosADL.BinaryExpression (Some l__max) (Some "-") (Some r__min)))) in Gamma
+      expression node (l - r)%sosadl
+                 has type [ l__min - r__max, l__max - r__min ]%sosadl in Gamma
 
 | type_expression_Mul:
     forall
@@ -787,20 +947,19 @@ with type_expression_node: env -> SosADL.SosADL.t_Expression -> SosADL.SosADL.t_
       (min: SosADL.SosADL.t_Expression)
       (max: SosADL.SosADL.t_Expression)
       (p1: expression l has type l__tau in Gamma)
-      (p2: l__tau </ (SosADL.SosADL.RangeType (Some l__min) (Some l__max)))
+      (p2: l__tau </ [l__min, l__max]%sosadl)
       (p3: expression r has type r__tau in Gamma)
-      (p4: r__tau </ (SosADL.SosADL.RangeType (Some r__min) (Some r__max)))
-      (p5: min <= (SosADL.SosADL.BinaryExpression (Some l__min) (Some "*") (Some r__min)))
-      (p6: min <= (SosADL.SosADL.BinaryExpression (Some l__min) (Some "*") (Some r__max)))
-      (p7: min <= (SosADL.SosADL.BinaryExpression (Some l__max) (Some "*") (Some r__min)))
-      (p8: min <= (SosADL.SosADL.BinaryExpression (Some l__max) (Some "*") (Some r__max)))
-      (p9: (SosADL.SosADL.BinaryExpression (Some l__min) (Some "*") (Some r__min)) <= max)
-      (pa: (SosADL.SosADL.BinaryExpression (Some l__min) (Some "*") (Some r__max)) <= max)
-      (pb: (SosADL.SosADL.BinaryExpression (Some l__max) (Some "*") (Some r__min)) <= max)
-      (pc: (SosADL.SosADL.BinaryExpression (Some l__max) (Some "*") (Some r__max)) <= max)
+      (p4: r__tau </ [r__min, r__max]%sosadl)
+      (p5: min <= (l__min * r__min)%sosadl)
+      (p6: min <= (l__min * r__max)%sosadl)
+      (p7: min <= (l__max * r__min)%sosadl)
+      (p8: min <= (l__max * r__max)%sosadl)
+      (p9: (l__min * r__min)%sosadl <= max)
+      (pa: (l__min * r__max)%sosadl <= max)
+      (pb: (l__max *  r__min)%sosadl <= max)
+      (pc: (l__max * r__max)%sosadl <= max)
     ,
-      expression node (SosADL.SosADL.BinaryExpression (Some l) (Some "*") (Some r))
-      has type (SosADL.SosADL.RangeType (Some min) (Some max)) in Gamma
+      expression node (l * r)%sosadl has type [min, max]%sosadl in Gamma
 
 | type_expression_Div_pos:
     forall
@@ -816,21 +975,20 @@ with type_expression_node: env -> SosADL.SosADL.t_Expression -> SosADL.SosADL.t_
       (min: SosADL.SosADL.t_Expression)
       (max: SosADL.SosADL.t_Expression)
       (p1: expression l has type l__tau in Gamma)
-      (p2: l__tau </ (SosADL.SosADL.RangeType (Some l__min) (Some l__max)))
+      (p2: l__tau </ [l__min, l__max]%sosadl)
       (p3: expression r has type r__tau in Gamma)
-      (p4: r__tau </ (SosADL.SosADL.RangeType (Some r__min) (Some r__max)))
+      (p4: r__tau </ [r__min, r__max]%sosadl)
       (p5: (SosADL.SosADL.IntegerValue (Some 1%Z)) <= r__min)
-      (p6: min <= (SosADL.SosADL.BinaryExpression (Some l__min) (Some "/") (Some r__min)))
-      (p7: min <= (SosADL.SosADL.BinaryExpression (Some l__min) (Some "/") (Some r__max)))
-      (p8: min <= (SosADL.SosADL.BinaryExpression (Some l__max) (Some "/") (Some r__min)))
-      (p9: min <= (SosADL.SosADL.BinaryExpression (Some l__max) (Some "/") (Some r__max)))
-      (pa: (SosADL.SosADL.BinaryExpression (Some l__min) (Some "/") (Some r__min)) <= max)
-      (pb: (SosADL.SosADL.BinaryExpression (Some l__min) (Some "/") (Some r__max)) <= max)
-      (pc: (SosADL.SosADL.BinaryExpression (Some l__max) (Some "/") (Some r__min)) <= max)
-      (pd: (SosADL.SosADL.BinaryExpression (Some l__max) (Some "/") (Some r__max)) <= max)
+      (p6: min <= (l__min / r__min)%sosadl)
+      (p7: min <= (l__min / r__max)%sosadl)
+      (p8: min <= (l__max / r__min)%sosadl)
+      (p9: min <= (l__max / r__max)%sosadl)
+      (pa: (l__min / r__min)%sosadl <= max)
+      (pb: (l__min / r__max)%sosadl <= max)
+      (pc: (l__max / r__min)%sosadl <= max)
+      (pd: (l__max / r__max)%sosadl <= max)
     ,
-      expression node (SosADL.SosADL.BinaryExpression (Some l) (Some "/") (Some r))
-      has type (SosADL.SosADL.RangeType (Some min) (Some max)) in Gamma
+      expression node (l / r)%sosadl has type [min, max]%sosadl in Gamma
 
 | type_expression_Div_neg:
     forall
@@ -846,21 +1004,20 @@ with type_expression_node: env -> SosADL.SosADL.t_Expression -> SosADL.SosADL.t_
       (min: SosADL.SosADL.t_Expression)
       (max: SosADL.SosADL.t_Expression)
       (p1: expression l has type l__tau in Gamma)
-      (p2: l__tau </ (SosADL.SosADL.RangeType (Some l__min) (Some l__max)))
+      (p2: l__tau </ [l__min, l__max]%sosadl)
       (p3: expression r has type r__tau in Gamma)
-      (p4: r__tau </ (SosADL.SosADL.RangeType (Some r__min) (Some r__max)))
-      (p5: (r__max <= (SosADL.SosADL.UnaryExpression (Some "-") (Some (SosADL.SosADL.IntegerValue (Some 1%Z))))))
-      (p6: min <= (SosADL.SosADL.BinaryExpression (Some l__min) (Some "/") (Some r__min)))
-      (p7: min <= (SosADL.SosADL.BinaryExpression (Some l__min) (Some "/") (Some r__max)))
-      (p8: min <= (SosADL.SosADL.BinaryExpression (Some l__max) (Some "/") (Some r__min)))
-      (p9: min <= (SosADL.SosADL.BinaryExpression (Some l__max) (Some "/") (Some r__max)))
-      (pa: (SosADL.SosADL.BinaryExpression (Some l__min) (Some "/") (Some r__min)) <= max)
-      (pb: (SosADL.SosADL.BinaryExpression (Some l__min) (Some "/") (Some r__max)) <= max)
-      (pc: (SosADL.SosADL.BinaryExpression (Some l__max) (Some "/") (Some r__min)) <= max)
-      (pd: (SosADL.SosADL.BinaryExpression (Some l__max) (Some "/") (Some r__max)) <= max)
+      (p4: r__tau </ [r__min, r__max]%sosadl)
+      (p5: (r__max <= (- (SosADL.SosADL.IntegerValue (Some 1%Z)))%sosadl))
+      (p6: min <= (l__min / r__min)%sosadl)
+      (p7: min <= (l__min / r__max)%sosadl)
+      (p8: min <= (l__max / r__min)%sosadl)
+      (p9: min <= (l__max / r__max)%sosadl)
+      (pa: (l__min / r__min)%sosadl <= max)
+      (pb: (l__min / r__max)%sosadl <= max)
+      (pc: (l__max / r__min)%sosadl <= max)
+      (pd: (l__max / r__max)%sosadl <= max)
     ,
-      expression node (SosADL.SosADL.BinaryExpression (Some l) (Some "/") (Some r))
-      has type (SosADL.SosADL.RangeType (Some min) (Some max)) in Gamma
+      expression node (l / r)%sosadl has type [min, max]%sosadl in Gamma
 
 | type_expression_Mod:
     forall
@@ -876,14 +1033,13 @@ with type_expression_node: env -> SosADL.SosADL.t_Expression -> SosADL.SosADL.t_
       (min: SosADL.SosADL.t_Expression)
       (max: SosADL.SosADL.t_Expression)
       (p1: expression l has type l__tau in Gamma)
-      (p2: l__tau </ (SosADL.SosADL.RangeType (Some l__min) (Some l__max)))
+      (p2: l__tau </ [l__min, l__max]%sosadl)
       (p3: expression r has type r__tau in Gamma)
-      (p4: r__tau </ (SosADL.SosADL.RangeType (Some r__min) (Some r__max)))
+      (p4: r__tau </ [r__min, r__max]%sosadl)
       (p5: range_modulo_min l__min l__max r__min r__max min)
       (p6: range_modulo_max l__min l__max r__min r__max max)
     ,
-      expression node (SosADL.SosADL.BinaryExpression (Some l) (Some "mod") (Some r))
-      has type (SosADL.SosADL.RangeType (Some min) (Some max)) in Gamma
+      expression node (l mod r)%sosadl has type [min, max]%sosadl in Gamma
 
 | type_expression_Implies:
     forall (Gamma: env)
@@ -896,7 +1052,7 @@ with type_expression_node: env -> SosADL.SosADL.t_Expression -> SosADL.SosADL.t_
       (p3: expression r has type r__tau in Gamma)
       (p4: r__tau </ SosADL.SosADL.BooleanType)
     ,
-     expression node (SosADL.SosADL.BinaryExpression (Some l) (Some "implies") (Some r)) has type SosADL.SosADL.BooleanType in Gamma
+     expression node (l -> r)%sosadl has type SosADL.SosADL.BooleanType in Gamma
 
 | type_expression_Or:
     forall (Gamma: env)
@@ -909,7 +1065,7 @@ with type_expression_node: env -> SosADL.SosADL.t_Expression -> SosADL.SosADL.t_
       (p3: expression r has type r__tau in Gamma)
       (p4: r__tau </ SosADL.SosADL.BooleanType)
     ,
-     expression node (SosADL.SosADL.BinaryExpression (Some l) (Some "or") (Some r)) has type SosADL.SosADL.BooleanType in Gamma
+     expression node (l || r)%sosadl has type SosADL.SosADL.BooleanType in Gamma
 
 | type_expression_Xor:
     forall (Gamma: env)
@@ -922,7 +1078,7 @@ with type_expression_node: env -> SosADL.SosADL.t_Expression -> SosADL.SosADL.t_
       (p3: expression r has type r__tau in Gamma)
       (p4: r__tau </ SosADL.SosADL.BooleanType)
     ,
-     expression node (SosADL.SosADL.BinaryExpression (Some l) (Some "xor") (Some r)) has type SosADL.SosADL.BooleanType in Gamma
+     expression node (l ^^ r)%sosadl has type SosADL.SosADL.BooleanType in Gamma
 
 | type_expression_And:
     forall (Gamma: env)
@@ -935,7 +1091,7 @@ with type_expression_node: env -> SosADL.SosADL.t_Expression -> SosADL.SosADL.t_
       (p3: expression r has type r__tau in Gamma)
       (p4: r__tau </ SosADL.SosADL.BooleanType)
     ,
-     expression node (SosADL.SosADL.BinaryExpression (Some l) (Some "and") (Some r)) has type SosADL.SosADL.BooleanType in Gamma
+     expression node (l && r)%sosadl has type SosADL.SosADL.BooleanType in Gamma
 
 | type_expression_Equal:
     forall (Gamma: env)
@@ -948,11 +1104,11 @@ with type_expression_node: env -> SosADL.SosADL.t_Expression -> SosADL.SosADL.t_
       (r__min: SosADL.SosADL.t_Expression)
       (r__max: SosADL.SosADL.t_Expression)
       (p1: expression l has type l__tau in Gamma)
-      (p2: l__tau </ SosADL.SosADL.RangeType (Some l__min) (Some l__max))
+      (p2: l__tau </ [l__min, l__max]%sosadl)
       (p3: expression r has type r__tau in Gamma)
-      (p4: r__tau </ SosADL.SosADL.RangeType (Some r__min) (Some r__max))
+      (p4: r__tau </ [r__min, r__max]%sosadl)
     ,
-      expression node (SosADL.SosADL.BinaryExpression (Some l) (Some "=") (Some r)) has type SosADL.SosADL.BooleanType in Gamma
+      expression node (l = r)%sosadl has type SosADL.SosADL.BooleanType in Gamma
 
 | type_expression_Diff:
     forall (Gamma: env)
@@ -965,11 +1121,11 @@ with type_expression_node: env -> SosADL.SosADL.t_Expression -> SosADL.SosADL.t_
       (r__min: SosADL.SosADL.t_Expression)
       (r__max: SosADL.SosADL.t_Expression)
       (p1: expression l has type l__tau in Gamma)
-      (p2: l__tau </ SosADL.SosADL.RangeType (Some l__min) (Some l__max))
+      (p2: l__tau </ [l__min, l__max]%sosadl)
       (p3: expression r has type r__tau in Gamma)
-      (p4: r__tau </ SosADL.SosADL.RangeType (Some r__min) (Some r__max))
+      (p4: r__tau </ [r__min, r__max]%sosadl)
     ,
-      expression node (SosADL.SosADL.BinaryExpression (Some l) (Some "<>") (Some r)) has type SosADL.SosADL.BooleanType in Gamma
+      expression node (l <> r)%sosadl has type SosADL.SosADL.BooleanType in Gamma
 
 | type_expression_Lt:
     forall (Gamma: env)
@@ -982,11 +1138,11 @@ with type_expression_node: env -> SosADL.SosADL.t_Expression -> SosADL.SosADL.t_
       (r__min: SosADL.SosADL.t_Expression)
       (r__max: SosADL.SosADL.t_Expression)
       (p1: expression l has type l__tau in Gamma)
-      (p2: l__tau </ SosADL.SosADL.RangeType (Some l__min) (Some l__max))
+      (p2: l__tau </ [l__min, l__max]%sosadl)
       (p3: expression r has type r__tau in Gamma)
-      (p4: r__tau </ SosADL.SosADL.RangeType (Some r__min) (Some r__max))
+      (p4: r__tau </ [r__min, r__max]%sosadl)
     ,
-      expression node (SosADL.SosADL.BinaryExpression (Some l) (Some "<") (Some r)) has type SosADL.SosADL.BooleanType in Gamma
+      expression node (l < r)%sosadl has type SosADL.SosADL.BooleanType in Gamma
 
 | type_expression_Le:
     forall (Gamma: env)
@@ -999,11 +1155,11 @@ with type_expression_node: env -> SosADL.SosADL.t_Expression -> SosADL.SosADL.t_
       (r__min: SosADL.SosADL.t_Expression)
       (r__max: SosADL.SosADL.t_Expression)
       (p1: expression l has type l__tau in Gamma)
-      (p2: l__tau </ SosADL.SosADL.RangeType (Some l__min) (Some l__max))
+      (p2: l__tau </ [l__min, l__max]%sosadl)
       (p3: expression r has type r__tau in Gamma)
-      (p4: r__tau </ SosADL.SosADL.RangeType (Some r__min) (Some r__max))
+      (p4: r__tau </ [r__min, r__max]%sosadl)
     ,
-      expression node (SosADL.SosADL.BinaryExpression (Some l) (Some "<=") (Some r)) has type SosADL.SosADL.BooleanType in Gamma
+      expression node (l <= r)%sosadl has type SosADL.SosADL.BooleanType in Gamma
 
 | type_expression_Gt:
     forall (Gamma: env)
@@ -1016,11 +1172,11 @@ with type_expression_node: env -> SosADL.SosADL.t_Expression -> SosADL.SosADL.t_
       (r__min: SosADL.SosADL.t_Expression)
       (r__max: SosADL.SosADL.t_Expression)
       (p1: expression l has type l__tau in Gamma)
-      (p2: l__tau </ SosADL.SosADL.RangeType (Some l__min) (Some l__max))
+      (p2: l__tau </ [l__min, l__max]%sosadl)
       (p3: expression r has type r__tau in Gamma)
-      (p4: r__tau </ SosADL.SosADL.RangeType (Some r__min) (Some r__max))
+      (p4: r__tau </ [r__min, r__max]%sosadl)
     ,
-      expression node (SosADL.SosADL.BinaryExpression (Some l) (Some ">") (Some r)) has type SosADL.SosADL.BooleanType in Gamma
+      expression node (l > r)%sosadl has type SosADL.SosADL.BooleanType in Gamma
 
 | type_expression_Ge:
     forall (Gamma: env)
@@ -1033,11 +1189,11 @@ with type_expression_node: env -> SosADL.SosADL.t_Expression -> SosADL.SosADL.t_
       (r__min: SosADL.SosADL.t_Expression)
       (r__max: SosADL.SosADL.t_Expression)
       (p1: expression l has type l__tau in Gamma)
-      (p2: l__tau </ SosADL.SosADL.RangeType (Some l__min) (Some l__max))
+      (p2: l__tau </ [l__min, l__max]%sosadl)
       (p3: expression r has type r__tau in Gamma)
-      (p4: r__tau </ SosADL.SosADL.RangeType (Some r__min) (Some r__max))
+      (p4: r__tau </ [r__min, r__max]%sosadl)
     ,
-      expression node (SosADL.SosADL.BinaryExpression (Some l) (Some ">=") (Some r)) has type SosADL.SosADL.BooleanType in Gamma
+      expression node (l >= r)%sosadl has type SosADL.SosADL.BooleanType in Gamma
 
 | type_expression_Ident:
     forall (Gamma: env)
@@ -1047,11 +1203,10 @@ with type_expression_node: env -> SosADL.SosADL.t_Expression -> SosADL.SosADL.t_
     ,
       expression node (SosADL.SosADL.IdentExpression (Some x)) has type tau in Gamma
 
-(** %\note{%According to the current implementation of environment, the
- rule [type_expression_MethodCall] accept any method declaration with
- the correct name and compatible parameter and [self] types. With this
- definition, the type checker can freely choose any such method
- declaration.%}% *)
+(** %\note{%The rule [type_expression_MethodCall] accept any method
+ declaration with the correct name and compatible parameter and [self]
+ types. With this definition, the type checker can freely choose any
+ such method declaration.%}% *)
 
 | type_expression_MethodCall:
     forall (Gamma: env)
@@ -1067,20 +1222,24 @@ with type_expression_node: env -> SosADL.SosADL.t_Expression -> SosADL.SosADL.t_
       (p1: expression self has type t in Gamma)
       (p2: binds Gamma (EType typeDecl tau methods))
       (p4: t </ tau)
-      (p5: method name defined in methods with tau parameters formalparams returns ret)
+      (p5: method name defined in methods
+       with tau parameters formalparams returns ret)
       (p6: for each fp p of formalparams params,
            (exists t, SosADL.SosADL.FormalParameter_type fp = Some t
                  /\ (exists tp, (expression p has type tp in Gamma)
                           /\ tp </ t)))
     ,
-      expression node (SosADL.SosADL.MethodCall (Some self) (Some name) params) has type ret in Gamma
+      expression node (SosADL.SosADL.MethodCall
+                         (Some self) (Some name) params)
+                 has type ret in Gamma
 
 
 | type_expression_Tuple:
     forall (Gamma: env)
       (elts: list SosADL.SosADL.t_TupleElement)
       (typ: list SosADL.SosADL.t_FieldDecl)
-      (p1: values (SosADL.SosADL.TupleElement_label x) for x of elts are distinct according to option_string_dec)
+      (p1: values (SosADL.SosADL.TupleElement_label x) for x of elts
+                  are distinct according to option_string_dec)
       (p2: for each e f of elts typ,
          SosADL.SosADL.TupleElement_label e = SosADL.SosADL.FieldDecl_name f)
       (p3: for each e f of elts typ,
@@ -1090,7 +1249,8 @@ with type_expression_node: env -> SosADL.SosADL.t_Expression -> SosADL.SosADL.t_
                 SosADL.SosADL.FieldDecl_type f = Some f'
                 /\ expression e' has type f' in Gamma))
     ,
-      expression node (SosADL.SosADL.Tuple elts) has type (SosADL.SosADL.TupleType typ) in Gamma
+      expression node (SosADL.SosADL.Tuple elts)
+                 has type (SosADL.SosADL.TupleType typ) in Gamma
 
 | type_expression_Field:
     forall (Gamma: env)
@@ -1101,7 +1261,7 @@ with type_expression_node: env -> SosADL.SosADL.t_Expression -> SosADL.SosADL.t_
       (p1: expression self has type (SosADL.SosADL.TupleType tau) in Gamma)
       (p2: field_type tau name = Some tau__f)
     ,
-      expression node (SosADL.SosADL.Field (Some self) (Some name)) has type tau__f in Gamma
+      expression node (self ::: name)%sosadl has type tau__f in Gamma
 
 | type_expression_Sequence:
     forall (Gamma: env)
@@ -1111,7 +1271,8 @@ with type_expression_node: env -> SosADL.SosADL.t_Expression -> SosADL.SosADL.t_
            exists t, (expression e has type t in Gamma)
                 /\ t </ tau)
     ,
-      expression node (SosADL.SosADL.Sequence elts) has type (SosADL.SosADL.SequenceType (Some tau)) in Gamma
+      expression node (SosADL.SosADL.Sequence elts)
+                 has type (SosADL.SosADL.SequenceType (Some tau)) in Gamma
 
 | type_expression_Map:
     forall (Gamma: env)
@@ -1123,7 +1284,8 @@ with type_expression_node: env -> SosADL.SosADL.t_Expression -> SosADL.SosADL.t_
       (p1: expression obj has type (SosADL.SosADL.SequenceType (Some tau)) in Gamma)
       (p2: expression e has type tau__e in Gamma [| x <- EVariable tau |])
     ,
-      expression node (SosADL.SosADL.Map (Some obj) (Some x) (Some e)) has type (SosADL.SosADL.SequenceType (Some tau__e)) in Gamma
+      expression node (obj :: { x -> e})%sosadl
+                 has type (SosADL.SosADL.SequenceType (Some tau__e)) in Gamma
 
 | type_expression_Select:
     forall (Gamma: env)
@@ -1132,12 +1294,11 @@ with type_expression_node: env -> SosADL.SosADL.t_Expression -> SosADL.SosADL.t_
       (x: string)
       (e: SosADL.SosADL.t_Expression)
       (p1: expression obj has type (SosADL.SosADL.SequenceType (Some tau)) in Gamma)
-      (p2: expression e has type SosADL.SosADL.BooleanType in Gamma [| x <- EVariable tau |])
+      (p2: expression e has type SosADL.SosADL.BooleanType
+        in Gamma [| x <- EVariable tau |])
     ,
-      expression node (SosADL.SosADL.Select (Some obj) (Some x) (Some e)) has type (SosADL.SosADL.SequenceType (Some tau)) in Gamma
-
-(** %\todo{%[CallExpression], [UnobservableValue], [Unify], [Relay]
-and [Quantify] are not handled yet, but they are not allowed in any kind of expression.%}% *)
+      expression node (obj :: { x | e})%sosadl
+                 has type (SosADL.SosADL.SequenceType (Some tau)) in Gamma
 
 where "'expression' e 'has' 'type' t 'in' Gamma" := (type_expression Gamma e t)
 and "'expression' 'node' e 'has' 'type' t 'in' Gamma" := (type_expression_node Gamma e t)
@@ -1146,7 +1307,16 @@ and "'expression' 'node' e 'has' 'type' t 'in' Gamma" := (type_expression_node G
 
 (** ** Conditional statements *)
 
-Inductive smallest: SosADL.SosADL.t_Expression -> SosADL.SosADL.t_Expression -> SosADL.SosADL.t_Expression -> Prop :=
+(** Unless conditional statements update the environment in each
+branch according to the tests being evaluated, range types are almost
+impractical. [condition_true] and [condition_false] aim at specifying
+a (rather naive) strategy to do this. These judgments rely on
+[smallest] (respectively [greatest]), which asserts that an expression
+is the minimum (respectively the maximum) of two given expression. *)
+
+Inductive smallest:
+  SosADL.SosADL.t_Expression
+  -> SosADL.SosADL.t_Expression -> SosADL.SosADL.t_Expression -> Prop :=
 | smallest_l:
     forall (m: SosADL.SosADL.t_Expression)
       (l: SosADL.SosADL.t_Expression)
@@ -1165,7 +1335,9 @@ Inductive smallest: SosADL.SosADL.t_Expression -> SosADL.SosADL.t_Expression -> 
       smallest m l r
 .
 
-Inductive greatest: SosADL.SosADL.t_Expression -> SosADL.SosADL.t_Expression -> SosADL.SosADL.t_Expression -> Prop :=
+Inductive greatest:
+  SosADL.SosADL.t_Expression
+  -> SosADL.SosADL.t_Expression -> SosADL.SosADL.t_Expression -> Prop :=
 | greatest_l:
     forall (m: SosADL.SosADL.t_Expression)
       (l: SosADL.SosADL.t_Expression)
@@ -1184,6 +1356,9 @@ Inductive greatest: SosADL.SosADL.t_Expression -> SosADL.SosADL.t_Expression -> 
       greatest m l r
 .
 
+(** [negated_comparison] returns the negation of a given comparison
+operator. *)
+
 Definition negated_comparison op :=
   match op with
   | "<" => Some ">="
@@ -1195,6 +1370,9 @@ Definition negated_comparison op :=
   | _ => None
   end.
 
+(** [symmetric_comparison] returns the symmetric operator of a given
+comparison operator. *)
+
 Definition symmetric_comparison op :=
   match op with
   | "<" => Some ">"
@@ -1205,6 +1383,21 @@ Definition symmetric_comparison op :=
   | "<>" => Some "<>"
   | _ => None
   end.
+
+(**
+- [condition_true] asserts the environment in the [then] branch of a conditional statement, i.e., assuming that a given condition evaluates to [true].
+- [condition_false] is similar to [condition_true], but for the [then] branch of a conditional statement, i.e., assuming that a given condition evaluates to [false].
+
+The supported condition forms are:
+- comparisons;
+- negation;
+- in [condition_true]: conjunction;
+- in [condition_false]: disjunction.
+
+Whenever a condition [x <= y] is found to surely hold in the branch, when [x] and [y] are variables, [x] and [y] are rebound such that the upper bound of [x] is updated to the upper bound of [y], and the lower bound of [y] is updated to the lower bound of [x]. The algorithm proceeds in the same way when either [x] or [y] is not a variable.
+
+%\note{%The non-determinism in the rules can make the algorithm never terminate, due to [condition_true_sym]. Though, it is quite easy to derive an effective algorithm from the rules.%}%
+*)
 
 Inductive condition_true: env -> SosADL.SosADL.t_Expression -> env -> Prop :=
 | condition_true_general:
@@ -1219,7 +1412,7 @@ Inductive condition_true: env -> SosADL.SosADL.t_Expression -> env -> Prop :=
       (Gamma1: env)
       (p1: condition_false Gamma c Gamma1)
     ,
-      condition_true Gamma (SosADL.SosADL.UnaryExpression (Some "not") (Some c)) Gamma
+      condition_true Gamma (! c)%sosadl Gamma
 
 | condition_true_and:
     forall (Gamma: env)
@@ -1230,7 +1423,7 @@ Inductive condition_true: env -> SosADL.SosADL.t_Expression -> env -> Prop :=
       (p1: condition_true Gamma c1 Gamma1)
       (p2: condition_true Gamma1 c2 Gamma2)
     ,
-      condition_true Gamma (SosADL.SosADL.BinaryExpression (Some c1) (Some "and") (Some c2)) Gamma2
+      condition_true Gamma (c1 && c2)%sosadl Gamma2
 
 | condition_true_lt:
     forall (Gamma: env)
@@ -1242,13 +1435,17 @@ Inductive condition_true: env -> SosADL.SosADL.t_Expression -> env -> Prop :=
       (r_min: SosADL.SosADL.t_Expression)
       (r_max: SosADL.SosADL.t_Expression)
       (Gamma1: env)
-      (p1: expression (SosADL.SosADL.IdentExpression (Some x)) has type (SosADL.SosADL.RangeType (Some x_min) (Some x_max)) in Gamma)
-      (p2: expression r has type (SosADL.SosADL.RangeType (Some r_min) (Some r_max)) in Gamma)
-      (p3: smallest x_max_ x_max (SosADL.SosADL.BinaryExpression (Some r_max) (Some "-") (Some (SosADL.SosADL.IntegerValue (Some 1%Z)))))
-      (p4: type (SosADL.SosADL.RangeType (Some x_min) (Some x_max_)) looks fine)
-      (p5: condition_true (Gamma [| x <- EVariable (SosADL.SosADL.RangeType (Some x_min) (Some x_max_)) |]) (SosADL.SosADL.BinaryExpression (Some r) (Some ">") (Some (SosADL.SosADL.IdentExpression (Some x)))) Gamma1)
+      (p1: expression (SosADL.SosADL.IdentExpression (Some x))
+                      has type [x_min, x_max]%sosadl in Gamma)
+      (p2: expression r has type [r_min, r_max]%sosadl in Gamma)
+      (p3: smallest x_max_
+                    x_max (r_max - (SosADL.SosADL.IntegerValue (Some 1%Z)))%sosadl)
+      (p4: type [x_min, x_max_]%sosadl looks fine)
+      (p5: condition_true (Gamma [| x <- EVariable [x_min, x_max_]%sosadl |])
+                          (r > (SosADL.SosADL.IdentExpression (Some x)))%sosadl
+                          Gamma1)
     ,
-      condition_true Gamma (SosADL.SosADL.BinaryExpression (Some (SosADL.SosADL.IdentExpression (Some x))) (Some "<") (Some r)) Gamma1
+      condition_true Gamma ((SosADL.SosADL.IdentExpression (Some x)) < r)%sosadl Gamma1
 
 | condition_true_le:
     forall (Gamma: env)
@@ -1260,13 +1457,16 @@ Inductive condition_true: env -> SosADL.SosADL.t_Expression -> env -> Prop :=
       (r_min: SosADL.SosADL.t_Expression)
       (r_max: SosADL.SosADL.t_Expression)
       (Gamma1: env)
-      (p1: expression (SosADL.SosADL.IdentExpression (Some x)) has type (SosADL.SosADL.RangeType (Some x_min) (Some x_max)) in Gamma)
-      (p2: expression r has type (SosADL.SosADL.RangeType (Some r_min) (Some r_max)) in Gamma)
+      (p1: expression (SosADL.SosADL.IdentExpression (Some x))
+                      has type [x_min, x_max]%sosadl in Gamma)
+      (p2: expression r has type [r_min, r_max]%sosadl in Gamma)
       (p3: smallest x_max_ x_max r_max)
-      (p4: type (SosADL.SosADL.RangeType (Some x_min) (Some x_max_)) looks fine)
-      (p5: condition_true (Gamma [| x <- EVariable (SosADL.SosADL.RangeType (Some x_min) (Some x_max_)) |]) (SosADL.SosADL.BinaryExpression (Some r) (Some ">=") (Some (SosADL.SosADL.IdentExpression (Some x)))) Gamma1)
+      (p4: type [x_min, x_max_]%sosadl looks fine)
+      (p5: condition_true (Gamma [| x <- EVariable [x_min, x_max_]%sosadl |])
+                          (r >= (SosADL.SosADL.IdentExpression (Some x)))%sosadl
+                          Gamma1)
     ,
-      condition_true Gamma (SosADL.SosADL.BinaryExpression (Some (SosADL.SosADL.IdentExpression (Some x))) (Some "<=") (Some r)) Gamma1
+      condition_true Gamma ((SosADL.SosADL.IdentExpression (Some x)) <= r)%sosadl Gamma1
 
 | condition_true_eq:
     forall (Gamma: env)
@@ -1279,14 +1479,18 @@ Inductive condition_true: env -> SosADL.SosADL.t_Expression -> env -> Prop :=
       (r_min: SosADL.SosADL.t_Expression)
       (r_max: SosADL.SosADL.t_Expression)
       (Gamma1: env)
-      (p1: expression (SosADL.SosADL.IdentExpression (Some x)) has type (SosADL.SosADL.RangeType (Some x_min) (Some x_max)) in Gamma)
-      (p2: expression r has type (SosADL.SosADL.RangeType (Some r_min) (Some r_max)) in Gamma)
+      (p1: expression (SosADL.SosADL.IdentExpression (Some x))
+                      has type [x_min, x_max]%sosadl in Gamma)
+      (p2: expression r has type [r_min, r_max]%sosadl in Gamma)
       (p3: greatest x_min_ x_min r_min)
       (p4: smallest x_max_ x_max r_max)
-      (p5: type (SosADL.SosADL.RangeType (Some x_min_) (Some x_max_)) looks fine)
-      (p6: condition_true (Gamma [| x <- EVariable (SosADL.SosADL.RangeType (Some x_min_) (Some x_max_)) |]) (SosADL.SosADL.BinaryExpression (Some r) (Some "=") (Some (SosADL.SosADL.IdentExpression (Some x)))) Gamma1)
+      (p5: type [x_min_, x_max_]%sosadl looks fine)
+      (p6: condition_true
+             (Gamma [| x <- EVariable [x_min_, x_max_]%sosadl |])
+             (r = (SosADL.SosADL.IdentExpression (Some x)))%sosadl
+             Gamma1)
     ,
-      condition_true Gamma (SosADL.SosADL.BinaryExpression (Some (SosADL.SosADL.IdentExpression (Some x))) (Some "=") (Some r)) Gamma1
+      condition_true Gamma ((SosADL.SosADL.IdentExpression (Some x)) = r)%sosadl Gamma1
 
 | condition_true_ge:
     forall (Gamma: env)
@@ -1298,13 +1502,16 @@ Inductive condition_true: env -> SosADL.SosADL.t_Expression -> env -> Prop :=
       (r_min: SosADL.SosADL.t_Expression)
       (r_max: SosADL.SosADL.t_Expression)
       (Gamma1: env)
-      (p1: expression (SosADL.SosADL.IdentExpression (Some x)) has type (SosADL.SosADL.RangeType (Some x_min) (Some x_max)) in Gamma)
-      (p2: expression r has type (SosADL.SosADL.RangeType (Some r_min) (Some r_max)) in Gamma)
+      (p1: expression (SosADL.SosADL.IdentExpression (Some x))
+                      has type [x_min, x_max]%sosadl in Gamma)
+      (p2: expression r has type [r_min, r_max]%sosadl in Gamma)
       (p3: greatest x_min_ x_min r_min)
-      (p4: type (SosADL.SosADL.RangeType (Some x_min_) (Some x_max)) looks fine)
-      (p5: condition_true (Gamma [| x <- EVariable (SosADL.SosADL.RangeType (Some x_min_) (Some x_max)) |]) (SosADL.SosADL.BinaryExpression (Some r) (Some "<=") (Some (SosADL.SosADL.IdentExpression (Some x)))) Gamma1)
+      (p4: type [x_min_, x_max]%sosadl looks fine)
+      (p5: condition_true (Gamma [| x <- EVariable [x_min_, x_max]%sosadl |])
+                          (r <= (SosADL.SosADL.IdentExpression (Some x)))%sosadl
+                          Gamma1)
     ,
-      condition_true Gamma (SosADL.SosADL.BinaryExpression (Some (SosADL.SosADL.IdentExpression (Some x))) (Some ">=") (Some r)) Gamma1
+      condition_true Gamma ((SosADL.SosADL.IdentExpression (Some x)) >= r)%sosadl Gamma1
 
 | condition_true_gt:
     forall (Gamma: env)
@@ -1316,13 +1523,17 @@ Inductive condition_true: env -> SosADL.SosADL.t_Expression -> env -> Prop :=
       (r_min: SosADL.SosADL.t_Expression)
       (r_max: SosADL.SosADL.t_Expression)
       (Gamma1: env)
-      (p1: expression (SosADL.SosADL.IdentExpression (Some x)) has type (SosADL.SosADL.RangeType (Some x_min) (Some x_max)) in Gamma)
-      (p2: expression r has type (SosADL.SosADL.RangeType (Some r_min) (Some r_max)) in Gamma)
-      (p3: greatest x_min_ x_min (SosADL.SosADL.BinaryExpression (Some r_min) (Some "+") (Some (SosADL.SosADL.IntegerValue (Some 1%Z)))))
-      (p4: type (SosADL.SosADL.RangeType (Some x_min_) (Some x_max)) looks fine)
-      (p5: condition_true (Gamma [| x <- EVariable (SosADL.SosADL.RangeType (Some x_min_) (Some x_max)) |]) (SosADL.SosADL.BinaryExpression (Some r) (Some "<") (Some (SosADL.SosADL.IdentExpression (Some x)))) Gamma1)
+      (p1: expression (SosADL.SosADL.IdentExpression (Some x))
+                      has type [x_min, x_max]%sosadl in Gamma)
+      (p2: expression r has type [r_min, r_max]%sosadl in Gamma)
+      (p3: greatest x_min_ x_min
+                    (r_min + (SosADL.SosADL.IntegerValue (Some 1%Z)))%sosadl)
+      (p4: type [x_min_, x_max]%sosadl looks fine)
+      (p5: condition_true (Gamma [| x <- EVariable [x_min_, x_max]%sosadl |])
+                          (r < (SosADL.SosADL.IdentExpression (Some x)))%sosadl
+                          Gamma1)
     ,
-      condition_true Gamma (SosADL.SosADL.BinaryExpression (Some (SosADL.SosADL.IdentExpression (Some x))) (Some ">") (Some r)) Gamma1
+      condition_true Gamma ((SosADL.SosADL.IdentExpression (Some x)) > r)%sosadl Gamma1
 
 | condition_true_sym:
     forall (Gamma: env)
@@ -1330,9 +1541,12 @@ Inductive condition_true: env -> SosADL.SosADL.t_Expression -> env -> Prop :=
       (op: string)
       (r: SosADL.SosADL.t_Expression)
       (Gamma1: env)
-      (p1: condition_true Gamma (SosADL.SosADL.BinaryExpression (Some r) (symmetric_comparison op) (Some l)) Gamma1)
+      (p1: condition_true
+             Gamma (SosADL.SosADL.BinaryExpression
+                      (Some r) (symmetric_comparison op) (Some l)) Gamma1)
     ,
-      condition_true Gamma (SosADL.SosADL.BinaryExpression (Some l) (Some op) (Some r)) Gamma1
+      condition_true
+        Gamma (SosADL.SosADL.BinaryExpression (Some l) (Some op) (Some r)) Gamma1
 
 with condition_false: env -> SosADL.SosADL.t_Expression -> env -> Prop :=
 | condition_false_general:
@@ -1347,7 +1561,7 @@ with condition_false: env -> SosADL.SosADL.t_Expression -> env -> Prop :=
       (Gamma1: env)
       (p1: condition_true Gamma c Gamma1)
     ,
-      condition_false Gamma (SosADL.SosADL.UnaryExpression (Some "not") (Some c)) Gamma
+      condition_false Gamma (! c)%sosadl Gamma
 
 | condition_false_or:
     forall (Gamma: env)
@@ -1358,7 +1572,7 @@ with condition_false: env -> SosADL.SosADL.t_Expression -> env -> Prop :=
       (p1: condition_false Gamma c1 Gamma1)
       (p2: condition_false Gamma1 c2 Gamma2)
     ,
-      condition_false Gamma (SosADL.SosADL.BinaryExpression (Some c1) (Some "or") (Some c2)) Gamma2
+      condition_false Gamma (c1 || c2)%sosadl Gamma2
 
 | condition_false_cmp:
     forall (Gamma: env)
@@ -1366,16 +1580,18 @@ with condition_false: env -> SosADL.SosADL.t_Expression -> env -> Prop :=
       (op: string)
       (r: SosADL.SosADL.t_Expression)
       (Gamma1: env)
-      (p1: condition_true Gamma (SosADL.SosADL.BinaryExpression (Some l) (negated_comparison op) (Some r)) Gamma1)
+      (p1: condition_true
+             Gamma (SosADL.SosADL.BinaryExpression
+                      (Some l) (negated_comparison op) (Some r)) Gamma1)
     ,
-      condition_false Gamma (SosADL.SosADL.BinaryExpression (Some l) (Some op) (Some r)) Gamma1
+      condition_false Gamma (SosADL.SosADL.BinaryExpression
+                               (Some l) (Some op) (Some r)) Gamma1
 .
 
 
 (** ** Mediator *)
 
-(** %\note{%By choice, the elements declared in the mediator are typed
-in order by the set rules for [type_mediatorblock].%}% *)
+(** %\todo{% %}% *)
 
 Inductive type_mediator: env -> SosADL.SosADL.t_MediatorDecl -> Prop :=
        (* TODO
@@ -1390,7 +1606,6 @@ Inductive type_mediator: env -> SosADL.SosADL.t_MediatorDecl -> Prop :=
 
 with type_mediatorblock: env -> SosADL.SosADL.t_MediatorDecl -> Prop :=
 
-  (** %\todo{%Data type declarations in mediators should be inspired from the rules for systems.%}% *)
   (* TODO
 | type_MediatorDecl_datatype:
     forall Gamma name d d_name l duties bhv assump assert,
@@ -1420,8 +1635,7 @@ with type_mediatorblock: env -> SosADL.SosADL.t_MediatorDecl -> Prop :=
        
 (** ** Architecture *)
 
-(** %\note{%By choice, the elements declared in the architecture are
-typed in order by the set rules for [type_architectureblock].%}% *)
+(** %\todo{% %}% *)
 
 with type_architecture: env -> SosADL.SosADL.t_ArchitectureDecl -> Prop :=
 (* TODO
@@ -1436,7 +1650,6 @@ with type_architecture: env -> SosADL.SosADL.t_ArchitectureDecl -> Prop :=
 *)
 with type_architectureblock: env -> SosADL.SosADL.t_ArchitectureDecl -> Prop :=
 
-  (** %\todo{%Data type declarations in architectures should be inspired from the rules for systems.%}% *)
   (* TODO
 | type_ArchitectureDecl_datatype:
     forall Gamma name d d_name l gates bhv a,
@@ -1470,19 +1683,19 @@ with type_architectureblock: env -> SosADL.SosADL.t_ArchitectureDecl -> Prop :=
 
 (** ** Architecture behavior*)
 
-(* %\todo{%TBD%}% *)
+(** %\todo{% %}% *)
 
 with type_archbehavior: env ->  SosADL.SosADL.t_ArchBehaviorDecl -> Prop :=
 
 (** ** Assertion *)
 
-(** %\todo{TBD}% *)
+(** %\todo{% %}% *)
 
 with type_assertion: env -> SosADL.SosADL.t_AssertionDecl -> Prop :=
 
 (** ** Protocol *)
 
-(** %\todo{TBD}% *)
+(** %\todo{% %}% *)
 
 with type_protocol: env -> SosADL.SosADL.t_ProtocolDecl -> Prop :=
 
@@ -1505,7 +1718,7 @@ and "'protocol' p 'well' 'typed' 'in' Gamma" := (type_protocol Gamma p)
   statements, i.e., they cannot be followed by any subsequent
   statement.
 
-- [Valuing], [AssertBehavior], [Action], [ForEachBehavior] and
+- [ValuingBehavior], [AssertBehavior], [Action], [ForEachBehavior] and
   [DoExprBehavior] are non-tail statements. They must mandatorily be
   followed by subsequent statement.
 
@@ -1516,22 +1729,32 @@ and "'protocol' p 'well' 'typed' 'in' Gamma" := (type_protocol Gamma p)
 
   At non-tail position, the [else] clause is optional and the branches
   must not contain any tail statement.  Futhermore, the typing rule
-  adjust the typing environment in each branch according to the
+  adjusts the typing environment in each branch according to the
   condition. See [condition_true] and [condition_false] for further
   details.
 
 - [ChooseBehavior] statements behave like [IfThenElseBehavior]
-  statements. Note that the rules for [ChooseBehavior] do not enforce any restriction on the branches, such as the usual requirement that each branch starts with a blocking communication statement.
+  statements. Note that the rules for [ChooseBehavior] do not enforce
+  any restriction on the branches, such as the usual requirement that
+  each branch starts with a blocking communication statement.
 
 The typing rules for behavior bodies are structured as follow:
 
 - [type_bodyprefix] types a single non-tail statement and synthetizes
   the new environment for subsequent statements.
-- [type_nonfinalbody] types a non-final body of statements, i.e., with no tail statement.
-- [type_finalbody] types a final body of statements, i.e., terminated by a tail statement.
-  *)
 
-Inductive type_bodyprefix: env -> SosADL.SosADL.t_BehaviorStatement -> env -> Prop :=
+- [type_nonfinalbody] types a non-final body of statements, i.e., with
+  no tail statement.
+
+- [type_finalbody] types a final body of statements, i.e., terminated
+  by a tail statement.
+
+[type_bodyprefix] and [type_nonfinalbody] are mutually recursive.
+
+ *)
+
+Inductive type_bodyprefix:
+  env -> SosADL.SosADL.t_BehaviorStatement -> env -> Prop :=
 
 | type_bodyprefix_DoExpr:
     forall
@@ -1542,6 +1765,8 @@ Inductive type_bodyprefix: env -> SosADL.SosADL.t_BehaviorStatement -> env -> Pr
     ,
       statement (SosADL.SosADL.DoExprBehavior (Some e)) well typed in Gamma yields to Gamma
 
+(** %\todo{%[type_bodyprefix_Valuing_inferred] and [type_Valuing_inferred] have to be deduplicated.%}% *)
+
 | type_bodyprefix_Valuing_inferred:
     forall
       (Gamma: env)
@@ -1550,7 +1775,10 @@ Inductive type_bodyprefix: env -> SosADL.SosADL.t_BehaviorStatement -> env -> Pr
       (tau__e: SosADL.SosADL.t_DataType)
       (p1: expression e has type tau__e in Gamma)
     ,
-      statement (SosADL.SosADL.ValuingBehavior (Some (SosADL.SosADL.Valuing (Some x) None (Some e)))) well typed in Gamma yields to (Gamma [| x <- EVariable tau__e |])
+      statement (SosADL.SosADL.ValuingBehavior (Some (valuing x = e)%sosadl))
+                well typed in Gamma yields to (Gamma [| x <- EVariable tau__e |])
+
+(** %\todo{%[type_bodyprefix_Valuing_typed] and [type_Valuing_typed] have to be deduplicated.%}% *)
 
 | type_bodyprefix_Valuing_typed:
     forall
@@ -1562,7 +1790,8 @@ Inductive type_bodyprefix: env -> SosADL.SosADL.t_BehaviorStatement -> env -> Pr
       (p1: expression e has type tau__e in Gamma)
       (p2: tau__e </ tau)
     ,
-      statement (SosADL.SosADL.ValuingBehavior (Some (SosADL.SosADL.Valuing (Some x) (Some tau) (Some e)))) well typed in Gamma yields to (Gamma [| x <- EVariable tau |])
+      statement (SosADL.SosADL.ValuingBehavior (Some (valuing x is tau = e)%sosadl))
+                well typed in Gamma yields to (Gamma [| x <- EVariable tau |])
 
 | type_bodyprefix_IfThenElse:
     forall
@@ -1578,12 +1807,13 @@ Inductive type_bodyprefix: env -> SosADL.SosADL.t_BehaviorStatement -> env -> Pr
                        (fun g e =>
                           exists (Gammae: env),
                             condition_false g c Gammae
-                            /\ (nonfinal body (SosADL.SosADL.Behavior_statements e) well typed in Gammae))
+                            /\ (nonfinal body (SosADL.SosADL.Behavior_statements e)
+                                        well typed in Gammae))
                        Gamma oe)
     ,
-      statement (SosADL.SosADL.IfThenElseBehavior (Some c) (Some (SosADL.SosADL.Behavior t)) oe)
-                well typed in Gamma
-                                yields to Gamma
+      statement (SosADL.SosADL.IfThenElseBehavior
+                   (Some c) (Some (SosADL.SosADL.Behavior t)) oe)
+                well typed in Gamma yields to Gamma
 
 | type_bodyprefix_Choose:
     forall (Gamma: env)
@@ -1604,11 +1834,14 @@ Inductive type_bodyprefix: env -> SosADL.SosADL.t_BehaviorStatement -> env -> Pr
       (p2: nonfinal body b well typed in Gamma [| x <- EVariable tau__x |])
       (p3: tau </ tau__x)
     ,
-      statement (SosADL.SosADL.ForEachBehavior (Some x) (Some vals) (Some (SosADL.SosADL.Behavior b))) well typed in Gamma yields to Gamma
+      statement (SosADL.SosADL.ForEachBehavior
+                   (Some x) (Some vals) (Some (SosADL.SosADL.Behavior b)))
+                well typed in Gamma yields to Gamma
 
 (** %\note{%[type_bodyprefix_Send] and [type_bodyprefix_Receive]
-assume that the complex name is a pair: gate-or-duty, connection.%}%
-*)
+assume that the complex name is a pair containing the name of a
+gate-or-duty, followed by the name of a connection within that
+gate-or-duty.%}% *)
 
 | type_bodyprefix_Send:
     forall (Gamma: env)
@@ -1626,8 +1859,9 @@ assume that the complex name is a pair: gate-or-duty, connection.%}%
       (p4: expression e has type tau__e in Gamma)
       (p5: tau__e </ conn__tau)
     ,
-      statement (SosADL.SosADL.Action (Some (SosADL.SosADL.ComplexName (gd :: conn :: nil)))
-                                      (Some (SosADL.SosADL.SendAction (Some e))))
+      statement (SosADL.SosADL.Action
+                   (Some (SosADL.SosADL.ComplexName [gd; conn]))
+                   (Some (SosADL.SosADL.SendAction (Some e))))
            well typed in Gamma yields to Gamma
 
 | type_bodyprefix_Receive:
@@ -1645,8 +1879,9 @@ assume that the complex name is a pair: gate-or-duty, connection.%}%
       (p3: mode_receive mode)
       (p4: Gamma1 = Gamma[| x <- EVariable conn__tau |])
     ,
-      statement (SosADL.SosADL.Action (Some (SosADL.SosADL.ComplexName (gd :: conn :: nil)))
-                                      (Some (SosADL.SosADL.ReceiveAction (Some x))))
+      statement (SosADL.SosADL.Action
+                   (Some (SosADL.SosADL.ComplexName [gd; conn]))
+                   (Some (SosADL.SosADL.ReceiveAction (Some x))))
                 well typed in Gamma
                                 yields to Gamma1
 
@@ -1662,13 +1897,7 @@ assume that the complex name is a pair: gate-or-duty, connection.%}%
       body (SosADL.SosADL.BehaviorStatement_TellAssertion (Some name) (Some e) :: l) well typed in Gamma
 *)
 
-(** The idea underpinning the [type_AskStatement] rule is to assume an
-environment [ee] in which all the (free) names of [e] are bound to
-some type. Then the type of [e] as well as of the following statements
-are done in [ee] merged in [Gamma]. *)
-
-                                                                                 (** *)
-  (*
+(*
 | type_AskStatement:
     forall Gamma name e ee l,
       (forall x, List.In x (names_of_expression e) <-> exists tau, contains ee x (EType tau))
@@ -1697,7 +1926,9 @@ with type_nonfinalbody: env -> list SosADL.SosADL.t_BehaviorStatement -> Prop :=
       (p2: nonfinal body l well typed in Gamma1)
     ,
       nonfinal body (s :: l) well typed in Gamma
-where "'statement' b 'well' 'typed' 'in' Gamma 'yields' 'to' Gamma1" := (type_bodyprefix Gamma b Gamma1)
+
+where "'statement' b 'well' 'typed' 'in' Gamma 'yields' 'to' Gamma1"
+        := (type_bodyprefix Gamma b Gamma1)
 and "'nonfinal' 'body' b 'well' 'typed' 'in' Gamma" := (type_nonfinalbody Gamma b)
 .
 
@@ -1709,8 +1940,7 @@ Inductive type_finalbody: env -> list SosADL.SosADL.t_BehaviorStatement -> Prop 
       (s: SosADL.SosADL.t_BehaviorStatement)
       (Gamma1: env)
       (l: list SosADL.SosADL.t_BehaviorStatement)
-      (p1: statement s
-                     well typed in Gamma yields to Gamma1)
+      (p1: statement s well typed in Gamma yields to Gamma1)
       (p2: final body l well typed in Gamma1)
     ,
       final body (s :: l) well typed in Gamma
@@ -1721,7 +1951,9 @@ Inductive type_finalbody: env -> list SosADL.SosADL.t_BehaviorStatement -> Prop 
       (b: list SosADL.SosADL.t_BehaviorStatement)
       (p1: nonfinal body b well typed in Gamma)
     ,
-      final body (SosADL.SosADL.RepeatBehavior (Some (SosADL.SosADL.Behavior b)) :: nil) well typed in Gamma
+      final body [SosADL.SosADL.RepeatBehavior
+                    (Some (SosADL.SosADL.Behavior b))]
+            well typed in Gamma
 
 | type_finalbody_IfThenElse_general:
     forall
@@ -1737,7 +1969,10 @@ Inductive type_finalbody: env -> list SosADL.SosADL.t_BehaviorStatement -> Prop 
       (p4: condition_false Gamma c Gammae)
       (p5: final body e well typed in Gammae)
     ,
-      final body (SosADL.SosADL.IfThenElseBehavior (Some c) (Some (SosADL.SosADL.Behavior t)) (Some (SosADL.SosADL.Behavior e)) :: nil)
+      final body [SosADL.SosADL.IfThenElseBehavior
+                    (Some c)
+                    (Some (SosADL.SosADL.Behavior t))
+                    (Some (SosADL.SosADL.Behavior e))]
            well typed in Gamma
 
 | type_finalbody_Choose:
@@ -1746,19 +1981,19 @@ Inductive type_finalbody: env -> list SosADL.SosADL.t_BehaviorStatement -> Prop 
       (p1: for each b of branches,
            final body (SosADL.SosADL.Behavior_statements b) well typed in Gamma)
     ,
-      final body (SosADL.SosADL.ChooseBehavior branches :: nil) well typed in Gamma
+      final body [SosADL.SosADL.ChooseBehavior branches] well typed in Gamma
 
 | type_finalbody_Done:
     forall
       (Gamma: env)
     ,
-      final body (SosADL.SosADL.DoneBehavior :: nil) well typed in Gamma
+      final body [SosADL.SosADL.DoneBehavior] well typed in Gamma
 
 | type_finalbody_RecursiveCall:
     forall
       (Gamma: env)
     ,
-      final body ((SosADL.SosADL.RecursiveCall nil) :: nil) well typed in Gamma
+      final body [SosADL.SosADL.RecursiveCall nil] well typed in Gamma
 
 where "'final' 'body' b 'well' 'typed' 'in' Gamma" := (type_finalbody Gamma b)
 .
@@ -1772,7 +2007,9 @@ Inductive type_behavior: env -> SosADL.SosADL.t_BehaviorDecl -> Prop :=
       (b: list SosADL.SosADL.t_BehaviorStatement)
       (p1: final body b well typed in Gamma)
     ,
-      behavior (SosADL.SosADL.BehaviorDecl (Some name) (Some (SosADL.SosADL.Behavior b))) well typed in Gamma
+      behavior (SosADL.SosADL.BehaviorDecl
+                  (Some name) (Some (SosADL.SosADL.Behavior b)))
+               well typed in Gamma
 
 where "'behavior' b 'well' 'typed' 'in' Gamma" := (type_behavior Gamma b)
 .
@@ -1781,13 +2018,28 @@ where "'behavior' b 'well' 'typed' 'in' Gamma" := (type_behavior Gamma b)
  ** Formal parameters
  *)
 
+(** Regardless the context where they appear, formal parameters enter
+the environment in no specific order. In addition, they cannot refer
+to each other. The typing rule therefore calls the generic
+[mutually_translate] rule.
+
+[formalParameter_to_EVariable] builds an environment item for a given
+formal parameter. *)
+
 Definition formalParameter_to_EVariable p :=
   match SosADL.SosADL.FormalParameter_type p with
   | None => None
   | Some t => Some (EVariable t)
   end.
 
-Inductive type_formalParameter: env -> SosADL.SosADL.t_FormalParameter -> SosADL.SosADL.t_FormalParameter -> env -> Prop :=
+(** [type_formalParameter] asserts that a formal parameter is
+correctly defined in a given environment. It synthetizes a new formal
+parameter in which the data type has been substituted according to
+[type_datatype]. *)
+
+Inductive type_formalParameter:
+  env -> SosADL.SosADL.t_FormalParameter
+  -> SosADL.SosADL.t_FormalParameter -> env -> Prop :=
 
 | type_FormalParameter_typed:
     forall (Gamma: env)
@@ -1797,36 +2049,34 @@ Inductive type_formalParameter: env -> SosADL.SosADL.t_FormalParameter -> SosADL
       (Gamma1: env)
       (p1: type t is t1 in Gamma)
     ,
-      type_formalParameter Gamma (SosADL.SosADL.FormalParameter (Some n) (Some t))
-                           (SosADL.SosADL.FormalParameter (Some n) (Some t1)) Gamma1
+      type_formalParameter
+        Gamma (SosADL.SosADL.FormalParameter (Some n) (Some t))
+        (SosADL.SosADL.FormalParameter (Some n) (Some t1)) Gamma1
 .
 
+(** [type_formalParameters] asserts that a list of formal parameters
+is correct in a given environment.  It synthetizes a new list of
+formal parameters in which the data types have been substituted
+according to [type_datatype]. This predicate invokes the generic
+[mutually_translate] judgment with the right parameters. *)
+
 Definition type_formalParameters Gamma l l1 Gamma1 :=
-  @mutually_translate _ type_formalParameter SosADL.SosADL.FormalParameter_name formalParameter_to_EVariable
+  @mutually_translate _ type_formalParameter
+                      SosADL.SosADL.FormalParameter_name
+                      formalParameter_to_EVariable
                       Gamma l l1 Gamma1.
 
-(*
-Definition type_formalParameters Gamma l l' Gamma1 :=
-  (for each p p' of l l',
-   SosADL.SosADL.FormalParameter_name p = SosADL.SosADL.FormalParameter_name p'
-   /\ exists t, SosADL.SosADL.FormalParameter_type p = Some t
-          /\ exists t', SosADL.SosADL.FormalParameter_type p' = Some t'
-                  /\ type t is t' in Gamma)
-  /\ @mutually _ (fun gamma p _ => True)
-              SosADL.SosADL.FormalParameter_name
-              formalParameter_to_EVariable
-              Gamma l' Gamma1.
-*)
+(** ** Connections *)
 
-(**
- ** Gates and duties
+(** Connections are typed similarly to formal parameters: they cannot
+refer to each other, and the order of the declarations is
+insignificant. [type_connection] states the typing rules for a single
+connection. [type_connections] invokes [mutually_translate] with the
+right parameters in order to type a list of connections. *)
 
-Gates and duties are typed in a similar way.
- *)
-
-(** *** Connection *)
-
-Inductive type_connection: env -> SosADL.SosADL.t_Connection -> SosADL.SosADL.t_Connection -> env -> Prop :=
+Inductive type_connection:
+  env -> SosADL.SosADL.t_Connection
+  -> SosADL.SosADL.t_Connection -> env -> Prop :=
 
 | type_Connection_simple:
     forall (Gamma: env)
@@ -1838,15 +2088,30 @@ Inductive type_connection: env -> SosADL.SosADL.t_Connection -> SosADL.SosADL.t_
       (Gamma1: env)
       (p1: type t is t1 in Gamma)
     ,
-      type_connection Gamma (SosADL.SosADL.Connection (Some k) (Some name) (Some m) (Some t))
-                      (SosADL.SosADL.Connection (Some k) (Some name) (Some m) (Some t1)) Gamma1
+      type_connection
+        Gamma (SosADL.SosADL.Connection (Some k) (Some name) (Some m) (Some t))
+        (SosADL.SosADL.Connection (Some k) (Some name) (Some m) (Some t1)) Gamma1
 .
 
 Definition type_connections Gamma l l1 Gamma1 :=
-  @mutually_translate _ type_connection SosADL.SosADL.Connection_name (fun x => Some (EConnection x))
+  @mutually_translate _ type_connection
+                      SosADL.SosADL.Connection_name
+                      (fun x => Some (EConnection x))
                       Gamma l l1 Gamma1.
+(** ** Gates and duties
 
-Inductive type_gate: env -> SosADL.SosADL.t_GateDecl -> SosADL.SosADL.t_GateDecl -> env -> Prop :=
+Gates and duties are typed in a similar way. The only difference
+follows from the fact that the former appear only in systems while the
+latter in mediators. Like formal parameters and connections, they
+cannot refer to each other, and the order of their declarations is
+insignificant. [type_gate] is the judgement for a single
+gate. [type_gates] uses [mutually_translate] in order to deal with a
+list of gates. *)
+
+Inductive type_gate:
+  env -> SosADL.SosADL.t_GateDecl
+  -> SosADL.SosADL.t_GateDecl -> env -> Prop :=
+  
 | type_GateDecl:
     forall (Gamma: env)
       (name: string)
@@ -1858,8 +2123,9 @@ Inductive type_gate: env -> SosADL.SosADL.t_GateDecl -> SosADL.SosADL.t_GateDecl
       (p1: type_connections Gamma conns conns1 Gamma2)
       (p2: protocol p well typed in Gamma2)
     ,
-      type_gate Gamma (SosADL.SosADL.GateDecl (Some name) conns (Some p))
-                (SosADL.SosADL.GateDecl (Some name) conns1 (Some p)) Gamma1
+      type_gate
+        Gamma (SosADL.SosADL.GateDecl (Some name) conns (Some p))
+        (SosADL.SosADL.GateDecl (Some name) conns1 (Some p)) Gamma1
 .
 
 Definition gateDecl_to_EGateOrDuty g :=
@@ -1867,7 +2133,9 @@ Definition gateDecl_to_EGateOrDuty g :=
 
 Definition type_gates Gamma l Gamma1 :=
   exists l1,
-    @mutually_translate _ type_gate SosADL.SosADL.GateDecl_name gateDecl_to_EGateOrDuty
+    @mutually_translate _ type_gate
+                        SosADL.SosADL.GateDecl_name
+                        gateDecl_to_EGateOrDuty
                         Gamma l l1 Gamma1.
 
 (*
@@ -1885,6 +2153,13 @@ where "'duty' d 'well' 'typed' 'in' Gamma" := (type_duty Gamma d)
 *)
 
 (** ** Valuings *)
+
+(** In a list, the valuings are handled one after the other, using
+[incrementally].
+
+When the type of a valuing is missing, the computed type of the
+expression is used instead.  *)
+
 Inductive type_valuing: env -> SosADL.SosADL.t_Valuing -> env -> Prop :=
 
 | type_Valuing_typed:
@@ -1896,7 +2171,7 @@ Inductive type_valuing: env -> SosADL.SosADL.t_Valuing -> env -> Prop :=
       (p1: expression e has type tau__e in Gamma)
       (p2: tau__e </ tau)
     ,
-      valuing (SosADL.SosADL.Valuing (Some x) (Some tau) (Some e))
+      valuing (valuing x is tau = e)%sosadl
               well typed in Gamma
                               yields to (Gamma [| x <- EVariable tau |])
 
@@ -1907,22 +2182,26 @@ Inductive type_valuing: env -> SosADL.SosADL.t_Valuing -> env -> Prop :=
       (tau__e: SosADL.SosADL.t_DataType)
       (p1: expression e has type tau__e in Gamma)
     ,
-      valuing (SosADL.SosADL.Valuing (Some x) None (Some e))
+      valuing (valuing x = e)%sosadl
               well typed in Gamma
                               yields to (Gamma [| x <- EVariable tau__e |])
 
-where "'valuing' v 'well' 'typed' 'in' Gamma 'yields' 'to' Gamma1" := (type_valuing Gamma v Gamma1)
+where "'valuing' v 'well' 'typed' 'in' Gamma 'yields' 'to' Gamma1"
+        := (type_valuing Gamma v Gamma1)
 .
 
 Definition type_valuings Gamma l Gamma1 := @incrementally _ type_valuing Gamma l Gamma1.
 
 (** ** Function declaration *)
 
+
+(** %\note{%Since the language does not allow conditional expression,
+permitting (mutually) recursive functions is irrelevant.%}% *)
+
+(** %\note{%Since the concrete grammar restricts all the functions to
+be methods, only this case is taken into account.%}% *)
+
 Inductive type_function: env -> SosADL.SosADL.t_FunctionDecl -> env -> Prop :=
-
-(** %\note{%Since the language does not allow conditional expression, permitting (mutually) recursive functions is irrelevant.%}% *)
-
-(** %\note{%Since the concrete grammar restricts all the functions to be methods, only this case is taken into account.%}% *)
 
 | type_FunctionDecl_Method:
     forall
@@ -1943,53 +2222,71 @@ Inductive type_function: env -> SosADL.SosADL.t_FunctionDecl -> env -> Prop :=
       (retexpr: SosADL.SosADL.t_Expression)
       (tau: SosADL.SosADL.t_DataType)
       (Gamma1: env)
-      (p1: Gamma [| dataTypeName |] = Some (EType dataTypeDecl dataTypeReal dataTypeMethods))
+      (p1: Gamma [| dataTypeName |] =
+           Some (EType dataTypeDecl dataTypeReal dataTypeMethods))
       (p2: type rettype is rettype' in Gamma)
-      (p3: type_formalParameters Gamma
-                                 (SosADL.SosADL.FormalParameter
-                                    (Some dataName)
-                                    (Some (SosADL.SosADL.NamedType (Some dataTypeName))) :: params)
-                                 (SosADL.SosADL.FormalParameter
-                                    (Some dataName)
-                                    (Some dataTypeReal) :: params')
-                                 Gammap)
+      (p3: type_formalParameters
+             Gamma
+             (SosADL.SosADL.FormalParameter
+                (Some dataName)
+                (Some (SosADL.SosADL.NamedType
+                         (Some dataTypeName))) :: params)
+             (SosADL.SosADL.FormalParameter
+                (Some dataName)
+                (Some dataTypeReal) :: params')
+             Gammap)
       (p4: type_valuings Gammap vals Gammav)
       (p5: expression retexpr has type tau in Gammav)
       (p6: tau </ rettype')
-      (p7: Gamma1 = Gamma [| dataTypeName <- EType dataTypeDecl dataTypeReal
-                                          ((SosADL.SosADL.FunctionDecl
-                                              (Some (SosADL.SosADL.FormalParameter
-                                                       (Some dataName)
-                                                       (Some dataTypeReal)))
-                                              (Some name) params' (Some rettype') vals (Some retexpr)) :: dataTypeMethods) |])
+      (p7: Gamma1 =
+           Gamma [| dataTypeName <- EType dataTypeDecl dataTypeReal
+                                 ((SosADL.SosADL.FunctionDecl
+                                     (Some (SosADL.SosADL.FormalParameter
+                                              (Some dataName)
+                                              (Some dataTypeReal)))
+                                     (Some name) params' (Some rettype')
+                                     vals (Some retexpr))
+                                    :: dataTypeMethods) |])
     ,
       function (SosADL.SosADL.FunctionDecl
                   (Some (SosADL.SosADL.FormalParameter
                            (Some dataName)
-                           (Some (SosADL.SosADL.NamedType (Some dataTypeName)))))
+                           (Some (SosADL.SosADL.NamedType
+                                    (Some dataTypeName)))))
                   (Some name) params (Some rettype) vals (Some retexpr))
                well typed in Gamma
                yields to Gamma1
 
-where "'function' f 'well' 'typed' 'in' Gamma 'yields' 'to' Gamma1" := (type_function Gamma f Gamma1)
+where "'function' f 'well' 'typed' 'in' Gamma 'yields' 'to' Gamma1"
+        := (type_function Gamma f Gamma1)
 .
 
 Definition type_functionDecls Gamma l Gamma1 := @incrementally _ type_function Gamma l Gamma1.
 
 (** ** Data type declaration *)
 
+(** In order to allow abstract (named) types despite the general
+approach based on structural typing, abstract (named) types are
+substituted by a uniquely generated named type. This approach avoids
+clashes and ensures the uniqueness of the abstract (named) types.
+
+[name_is_fresh] yields [true] if a name is fresh in a given
+environment. *)
+
 Fixpoint name_is_fresh (e: env) (x: string): bool :=
   match e with
   | h :: r =>
     andb
     match (value h) with
-    | EType _ (SosADL.SosADL.NamedType (Some n)) _ => (negb (string_eqb x n))
+    | EType _ (SosADL.SosADL.NamedType (Some n)) _ =>
+      (negb (string_eqb x n))
     | _ => true
     end (name_is_fresh r x)
   | nil => true
   end.
 
-Inductive type_datatypeDecl: env -> SosADL.SosADL.t_DataTypeDecl -> env -> Prop :=
+Inductive type_datatypeDecl:
+  env -> SosADL.SosADL.t_DataTypeDecl -> env -> Prop :=
 | type_DataTypeDecl_def:
     forall
       (Gamma: env)
@@ -2002,10 +2299,16 @@ Inductive type_datatypeDecl: env -> SosADL.SosADL.t_DataTypeDecl -> env -> Prop 
       (p2: for each f of funs,
            exists p,
              SosADL.SosADL.FunctionDecl_data f = Some p
-             /\ SosADL.SosADL.FormalParameter_type p = Some (SosADL.SosADL.NamedType (Some name)))
-      (p3: type_functionDecls (Gamma [| name <- EType (SosADL.SosADL.DataTypeDecl (Some name) (Some t) funs) t' nil |]) funs Gamma1)
+             /\ SosADL.SosADL.FormalParameter_type p
+               = Some (SosADL.SosADL.NamedType (Some name)))
+      (p3: type_functionDecls
+             (Gamma [| name <- EType
+                            (SosADL.SosADL.DataTypeDecl
+                               (Some name) (Some t) funs)
+                            t' nil |]) funs Gamma1)
     ,
-      typedecl (SosADL.SosADL.DataTypeDecl (Some name) (Some t) funs) well typed in Gamma yields to Gamma1
+      typedecl (SosADL.SosADL.DataTypeDecl (Some name) (Some t) funs)
+               well typed in Gamma yields to Gamma1
 
 | type_DataTypeDecl_def_None:
     forall
@@ -2018,20 +2321,26 @@ Inductive type_datatypeDecl: env -> SosADL.SosADL.t_DataTypeDecl -> env -> Prop 
       (p2: for each f of funs,
            exists p,
              SosADL.SosADL.FunctionDecl_data f = Some p
-             /\ SosADL.SosADL.FormalParameter_type p = Some (SosADL.SosADL.NamedType (Some name)))
-      (p3: type_functionDecls (Gamma [| name <- EType (SosADL.SosADL.DataTypeDecl (Some name) None funs) (SosADL.SosADL.NamedType (Some name')) nil |]) funs Gamma1)
+             /\ SosADL.SosADL.FormalParameter_type p
+               = Some (SosADL.SosADL.NamedType (Some name)))
+      (p3: type_functionDecls
+             (Gamma [| name <- EType
+                            (SosADL.SosADL.DataTypeDecl
+                               (Some name) None funs)
+                            (SosADL.SosADL.NamedType (Some name'))
+                            nil |]) funs Gamma1)
     ,
-      typedecl (SosADL.SosADL.DataTypeDecl (Some name) None funs) well typed in Gamma yields to Gamma1
+      typedecl (SosADL.SosADL.DataTypeDecl (Some name) None funs)
+               well typed in Gamma yields to Gamma1
 
-where "'typedecl' t 'well' 'typed' 'in' Gamma 'yields' 'to' Gamma1" := (type_datatypeDecl Gamma t Gamma1)
+where "'typedecl' t 'well' 'typed' 'in' Gamma 'yields' 'to' Gamma1"
+        := (type_datatypeDecl Gamma t Gamma1)
 .
 
-Definition type_datatypeDecls Gamma l Gamma1 := @incrementally _ type_datatypeDecl Gamma l Gamma1.
+Definition type_datatypeDecls Gamma l Gamma1 :=
+  @incrementally _ type_datatypeDecl Gamma l Gamma1.
 
 (** ** System *)
-
-(** %\note{%By choice, the elements declared in the system are typed
-in order by the set rules for [type_systemblock].%}% *)
 
 Inductive type_system: env -> SosADL.SosADL.t_SystemDecl -> Prop :=
 | type_SystemDecl:
@@ -2053,23 +2362,36 @@ Inductive type_system: env -> SosADL.SosADL.t_SystemDecl -> Prop :=
       (p4: behavior bhv well typed in Gamma3)
       (p5: @optionally _ (fun g a => assertion a well typed in g) Gamma3 assrt)
     ,
-      system (SosADL.SosADL.SystemDecl (Some name) params datatypes gates (Some bhv) assrt) well typed in Gamma
+      system (SosADL.SosADL.SystemDecl
+                (Some name) params datatypes gates (Some bhv) assrt)
+             well typed in Gamma
+
 where "'system' s 'well' 'typed' 'in' Gamma" := (type_system Gamma s)
 .
 
-Definition type_systems Gamma l Gamma1 := @incrementally _ (simple_increment _ type_system SosADL.SosADL.SystemDecl_name (fun x => Some (ESystem x))) Gamma l Gamma1.
+Definition type_systems Gamma l Gamma1 :=
+  @incrementally _ (simple_increment _ type_system
+                                     SosADL.SosADL.SystemDecl_name
+                                     (fun x => Some (ESystem x)))
+                 Gamma l Gamma1.
 
-Definition type_mediators Gamma l Gamma1 := @incrementally _ (simple_increment _ type_mediator SosADL.SosADL.MediatorDecl_name (fun x => Some (EMediator x))) Gamma l Gamma1.
-Definition type_architectures Gamma l Gamma1 := @incrementally _ (simple_increment _ type_architecture SosADL.SosADL.ArchitectureDecl_name (fun x => Some (EArchitecture x))) Gamma l Gamma1.
+Definition type_mediators Gamma l Gamma1 :=
+  @incrementally _ (simple_increment _ type_mediator
+                                     SosADL.SosADL.MediatorDecl_name
+                                     (fun x => Some (EMediator x)))
+                 Gamma l Gamma1.
+Definition type_architectures Gamma l Gamma1 :=
+  @incrementally _ (simple_increment _ type_architecture
+                                     SosADL.SosADL.ArchitectureDecl_name
+                                     (fun x => Some (EArchitecture x)))
+                 Gamma l Gamma1.
 
 (** ** Entity *)
 
-(** %\note{%We choose that the order of the declaration is
-significant for the typing rules. Namely, the scope of a declaration
-starts after this declaration and spans until the end of the enclosing
-block. This choice prevents, e.g., (mutually) recursive
-declarations. This behavior is implemented by the following rules,
-each of which exhausts of list of declarations in order.%}% *)
+(** The order of the declaration is significant for the typing
+rules. Namely, the scope of a declaration starts after this
+declaration and spans until the end of the enclosing block. This
+choice prevents, e.g., (mutually) recursive declarations. *)
 
 Inductive type_entityBlock: env -> SosADL.SosADL.t_EntityBlock -> Prop :=
 | type_EntityBlock_whole:
@@ -2091,7 +2413,9 @@ Inductive type_entityBlock: env -> SosADL.SosADL.t_EntityBlock -> Prop :=
       (p4: type_mediators Gamma3 mediators Gamma4)
       (p5: type_architectures Gamma4 architectures Gamma5)
     ,
-      entity (SosADL.SosADL.EntityBlock datatypes funs systems mediators architectures) well typed in Gamma
+      entity (SosADL.SosADL.EntityBlock
+                datatypes funs systems mediators architectures)
+             well typed in Gamma
   
 where "'entity' u 'well' 'typed' 'in' Gamma" := (type_entityBlock Gamma u)
 .
