types/coq/make-allpdf.sh
@@ -3,5 +3,6 @@
 rm -f all.pdf
 make -j2 &&
     find SosADL -name '*.v' | xargs coqdep -c -sort -suffix .v | xargs coqdoc -toc -interpolate -utf8 -latex -p "\usepackage{listings}" -o all.tex &&
+    sed -i.bak -e 's/\\usepackage{coqdoc}/\\usepackage[color]{coqdoc}/' all.tex &&
     latexmk -pdf all.tex
 
